1) proved the semantics-preservation of DIE. The version completed semantics- preservation of all passes except phinode elimination.
2) die.v was split into die_wfS.v die.v and die_top.v.



git-svn-id: https://webdav.seas.upenn.edu/svn/sol/vol@3933 eef5ea85-cc2e-0410-bd84-0fae1f012da8

src3.0/Transforms/die.v
@@ -7,27 +7,33 @@ Require Import Iteration.
 Require Import Maps.
 Require Import opsem_props.
 Require Import primitives.
+Require Import memory_sim.
+Require Import memory_props.
 Require Import program_sim.
 Require Import palloca_props.
 Require Import top_sim.
 Require Import trans_tactic.
 
-Definition pure_cmd (c:cmd) : Prop :=
-match c with
-| insn_free _ _ _
-| insn_alloca _ _ _ _
-| insn_malloc _ _ _ _
-| insn_store _ _ _ _ _
-| insn_call _ _ _ _ _ _ _ => False
-| _ => True
+Definition pure_cmd (instr:insn) : Prop :=
+match instr with
+| insn_cmd c =>
+  match c with
+  | insn_free _ _ _
+  | insn_alloca _ _ _ _
+  | insn_malloc _ _ _ _
+  | insn_store _ _ _ _ _
+  | insn_call _ _ _ _ _ _ _ => False
+  | _ => True
+  end
+| _ => False
 end.
 
 Record DIInfo := mkDIInfo {
   DI_f : fdef;
   DI_id : id;
-  DI_pure : forall c,
-               lookupInsnViaIDFromFdef DI_f DI_id = Some (insn_cmd c) ->
-               pure_cmd c;
+  DI_pure : forall instr,
+               lookupInsnViaIDFromFdef DI_f DI_id = Some instr ->
+               pure_cmd instr;
   DI_unused : used_in_fdef DI_id DI_f = false
 }.
 
@@ -131,6 +137,18 @@ Proof.
       destruct_dec. inv Hprop.
 Qed.
 
+Lemma dont_remove_phinodes: forall (dinfo : DIInfo) (ps1 : phinodes)
+  (l1 : l) (cs1 : cmds) (tmn1 : terminator)
+  (HBinF : blockInFdefB (block_intro l1 ps1 cs1 tmn1) (DI_f dinfo) = true)
+  (H : uniqFdef (DI_f dinfo)),
+  ~ In (DI_id dinfo) (getPhiNodesIDs ps1).
+Proof.
+  intros. intro Hin.
+  eapply IngetPhiNodesIDs__lookupPhinodeViaIDFromFdef in Hin; eauto.
+  destruct Hin as [p2 [Hin Heq]].
+  apply (DI_pure dinfo) in Hin. auto.
+Qed.
+
 Definition phis_simulation (dinfo: DIInfo) (f1:fdef) ps1 ps2 : Prop :=
 RemoveSim.phis_simulation (DI_f dinfo) (DI_id dinfo) f1 ps1 ps2.
 
@@ -141,12 +159,12 @@ Lemma phis_simulation_inv: forall dinfo F ps1 ps2 l1 cs1 tmn1
 Proof.
   intros.
   eapply RemoveSim.phis_simulation_inv; eauto 1.
-    intro. subst. admit. (* phicannot be removed *)
+    intro. subst. 
+    eapply dont_remove_phinodes; eauto.
 Qed.
 
 (* regsim can also be generalized *)
-Lemma reg_simulation_update_non_dead: forall dinfo F lc1 lc2 id0 gvs,
-  DI_f dinfo <> F \/ DI_id dinfo <> id0 ->
+Lemma reg_simulation_update: forall dinfo F lc1 lc2 id0 gvs,
   reg_simulation dinfo F lc1 lc2 ->
   reg_simulation dinfo F (updateAddAL (GVsT DGVs) lc1 id0 gvs)
     (updateAddAL (GVsT DGVs) lc2 id0 gvs).
@@ -154,8 +172,6 @@ Proof.
   unfold reg_simulation.
   intros.
   destruct (fdef_dec (DI_f dinfo) F); subst; intros; auto.
-    assert (J:=@H0 i0). clear H0.
-    destruct H as [H | H]; try congruence.
     destruct (id_dec id0 i0); subst.
       rewrite lookupAL_updateAddAL_eq; auto.
       rewrite lookupAL_updateAddAL_eq; auto.
@@ -211,7 +227,7 @@ Proof.
       eauto.
     erewrite simulation__getOperandValue in HeqR0; eauto.
       repeat uniq_result. 
-      apply reg_simulation_update_non_dead; auto.
+      apply reg_simulation_update; auto.
 
       destruct B2. simpl in HeqR3.
       assert (DI_f dinfo <> F \/ used_in_list_value_l (DI_id dinfo) l0 = false)
@@ -245,7 +261,8 @@ Proof.
   unfold Opsem.switchToNewBasicBlock in *. simpl in *.
   inv_mbind'. symmetry_ctx.
   eapply getIncomingValuesForBlockFromPHINodes_rsim; eauto.
-    admit. (* phi isnt dead *)
+    destruct (fdef_dec (DI_f dinfo) F); subst; auto.
+      right. eapply dont_remove_phinodes; eauto.
 Qed.
 
 Definition list_value_doesnt_use_did dinfo F idxs :=
@@ -286,9 +303,7 @@ Definition args_dont_use_did dinfo F (la:list (typ * attributes * id)) :=
   conditional_used_in_args (DI_f dinfo) F (DI_id dinfo) la.
 
 Lemma reg_simulation__initializeFrameValues: forall dinfo fa0 rt0 fid0 va0
-    TD lb la2 la1 (gvs:list (GVsT DGVs)) lc1 lc2 lc1' lc2'
-  (Hnuse: args_dont_use_did dinfo
-            (fdef_intro (fheader_intro fa0 rt0 fid0 (la1++la2) va0) lb) la2),
+    TD lb la2 la1 (gvs:list (GVsT DGVs)) lc1 lc2 lc1' lc2',
   reg_simulation dinfo 
     (fdef_intro (fheader_intro fa0 rt0 fid0 (la1++la2) va0) lb) lc1 lc2 ->
   Opsem._initializeFrameValues TD la2 gvs lc1 = ret lc1' ->
@@ -299,33 +314,14 @@ Proof.
   induction la2 as [|[[]]]; simpl; intros.
     uniq_result. auto.
 
-    assert (args_dont_use_did dinfo
-       (fdef_intro
-          (fheader_intro fa0 rt0 fid0 ((la1 ++ [(t, a, i0)]) ++ la2) va0) lb)
-       la2) as J.
-      unfold args_dont_use_did. unfold args_dont_use_did in Hnuse.
-      simpl_env. simpl_env in Hnuse.
-      destruct Hnuse as [Hnuse | Hnuse]; auto.
-      right.
-      intros.
-      eapply Hnuse; simpl; eauto.
-
-    assert (DI_f dinfo <>
-      fdef_intro (fheader_intro fa0 rt0 fid0 (la1 ++ (t, a, i0) :: la2) va0) lb\/
-      DI_id dinfo <> i0) as J'.
-      unfold args_dont_use_did in Hnuse.
-      destruct Hnuse as [Hnuse | Hnuse]; auto.
-      right.
-      eapply Hnuse; simpl; eauto.
-
     rewrite_env ((la1 ++ [(t, a, i0)]) ++ la2) in H.
     destruct gvs; inv_mbind''; symmetry_ctx.
       eapply IHla2 in H; eauto.
-        apply reg_simulation_update_non_dead; auto.
+        apply reg_simulation_update; auto.
         simpl_env in *. auto.
 
       eapply IHla2 in H; eauto.
-        apply reg_simulation_update_non_dead; auto.
+        apply reg_simulation_update; auto.
         simpl_env in *. auto.
 Qed.
 
@@ -338,9 +334,7 @@ Qed.
 
 Lemma reg_simulation__initLocals: forall dinfo F lc1 lc2 lp gl gvs1 gvs2 lc1'
   lc2' la los nts fa0 rt0 fid0 va0 lb 
-  (Hnuse: params_dont_use_did dinfo F lp)
-  (Hnuse': args_dont_use_did dinfo
-            (fdef_intro (fheader_intro fa0 rt0 fid0 la va0) lb) la),
+  (Hnuse: params_dont_use_did dinfo F lp),
   reg_simulation dinfo F lc1 lc2 ->
   Opsem.params2GVs (los,nts) lp lc1 gl = ret gvs1 ->
   Opsem.params2GVs (los,nts) lp lc2 gl = ret gvs2 ->
@@ -356,6 +350,70 @@ Proof.
   rewrite_env (nil++la).
   eapply reg_simulation__initializeFrameValues; eauto.
   apply reg_simulation_nil; auto.
+Qed.
+
+Lemma reg_simulation_update_dead: forall (dinfo : DIInfo)
+  (lc1 lc2 : Opsem.GVsMap) gv
+  (Hlcsim2 : reg_simulation dinfo (DI_f dinfo) lc1 lc2),
+  reg_simulation dinfo (DI_f dinfo)
+    (updateAddAL (GVsT DGVs) lc1 (DI_id dinfo) gv) lc2.
+Proof.
+  intros.
+  unfold reg_simulation in *.
+  destruct (fdef_dec (DI_f dinfo) (DI_f dinfo)); try congruence.
+  intros.
+  assert (J:=@Hlcsim2 i0). clear Hlcsim2.
+  rewrite <- lookupAL_updateAddAL_neq; auto.
+Qed.
+
+Lemma returnUpdateLocals_reg_simulation: forall dinfo F' lc' los nts i0 n
+  c t0 v0 v p Result lc gl lc'' lc3 lc''0 lc2 F 
+  (Hprop: DI_f dinfo <> F' \/ DI_id dinfo <> i0)
+  (Hprop': value_doesnt_use_did dinfo F Result)
+  (Hsim: reg_simulation dinfo F' lc' lc3)
+  (Hsim': reg_simulation dinfo F lc lc2)
+  (Hupdate: Opsem.returnUpdateLocals (los,nts) 
+              (insn_call i0 n c t0 v0 v p) Result lc lc' gl = ret lc'')
+  (Hupdate': Opsem.returnUpdateLocals (los,nts) 
+               (insn_call i0 n c t0 v0 v p) Result lc2 lc3 gl = ret lc''0),
+  reg_simulation dinfo F' lc'' lc''0.
+Proof.
+  intros.
+  unfold Opsem.returnUpdateLocals in *.
+  inv_mbind'. symmetry_ctx.
+  erewrite <- simulation__getOperandValue in HeqR; eauto.
+  destruct n; uniq_result; auto.
+  inv_mbind'. inv H0.
+  apply reg_simulation_update; auto.
+Qed.
+
+Lemma exCallUpdateLocals_reg_simulation: forall diinfo F lc1 lc2 lc1' lc2' td
+  rt1 noret0 rid oresult0 (Hlcsim2 : reg_simulation diinfo F lc1 lc2)
+  (H1: Opsem.exCallUpdateLocals td rt1 noret0 rid oresult0 lc1 = ret lc1')
+  (H2: Opsem.exCallUpdateLocals td rt1 noret0 rid oresult0 lc2 = ret lc2'),
+  reg_simulation diinfo F lc1' lc2'.
+Proof.
+  intros.
+  unfold Opsem.exCallUpdateLocals in *.
+  destruct_if.
+    uniq_result. auto.
+    inv_mbind; auto.
+    inv H1.
+    apply reg_simulation_update; auto.
+Qed.
+
+Lemma dont_remove_impure_cmd: forall (dinfo : DIInfo) (ps1 : phinodes)
+  (l1 : l) (cs1 : cmds) (tmn1 : terminator) F c cs0
+  (HBinF : blockInFdefB (block_intro l1 ps1 (cs0++c::cs1) tmn1) F = true)
+  (H : uniqFdef F) (Hnok: ~ pure_cmd (insn_cmd c)),
+  DI_f dinfo <> F \/ DI_id dinfo <> getCmdLoc c.
+Proof.
+  intros.
+  destruct (fdef_dec (DI_f dinfo) F); subst; auto.
+  right.
+  eapply IngetCmdsIDs__lookupCmdViaIDFromFdef in HBinF; eauto using in_middle.
+  intro EQ. rewrite <- EQ in HBinF.
+  apply (DI_pure dinfo) in HBinF. auto.
 Qed.
 
 Ltac destruct_ctx_other :=
@@ -376,7 +434,7 @@ match goal with
             OpsemAux.Globals := _;
             OpsemAux.FunTable := _
              |} _,
-  Hsim : State_simulation _ _ _ _ _ ?Cfg2 ?St2 ,
+  Hsim : State_simulation _ _ _ ?Cfg2 ?St2 ,
   Hop2 : Opsem.sInsn _ _ _ _ |- _ =>
   destruct TD as [los nts];
   destruct Hwfcfg as [_ [Hwfg [HwfSystem HmInS]]];
@@ -417,7 +475,7 @@ match goal with
             OpsemAux.Globals := _;
             OpsemAux.FunTable := _
              |} _,
-  Hsim : State_simulation _ _ _ _ _ ?Cfg2 ?St2 ,
+  Hsim : State_simulation _ _ _ ?Cfg2 ?St2 ,
   Hop2 : Opsem.sInsn _ _ _ _ |- _ =>
   destruct TD as [los nts];
   destruct Hwfcfg as [_ [Hwfg [HwfSystem HmInS]]];
@@ -454,8 +512,209 @@ end.
 Definition removable_State (dinfo: DIInfo) (St:@Opsem.State DGVs) : Prop :=
 RemoveSim.removable_State (DI_f dinfo) (DI_id dinfo) St.
 
+Lemma removable_State_inv': forall F0 ID0 St,
+  RemoveSim.removable_State F0 ID0 St ->
+  exists F, exists b, exists c, exists cs, exists tmn, exists lc, 
+    exists als, exists ECs, exists M,
+      St = {| Opsem.ECS := 
+                {| Opsem.CurFunction := F;
+                   Opsem.CurBB := b;
+                   Opsem.CurCmds := c :: cs;
+                   Opsem.Terminator := tmn;
+                   Opsem.Locals := lc;
+                   Opsem.Allocas := als |} :: ECs;
+              Opsem.Mem := M |} /\
+      F0 = F /\ ID0 = getCmdLoc c.
+Proof.
+  intros.
+  destruct St as [[|[? ? [|] ? ?]] ?]; tinv H.
+  apply RemoveSim.removable_State_inv in H. 
+  eauto 11.
+Qed.
+
+Ltac solve_lookupCmdViaIDFromFdef:=
+match goal with
+| Huniq: uniqFdef ?f,
+  H : blockInFdefB (block_intro _ _ (_++?c::_) _) ?f = true |- 
+  lookupInsnViaIDFromFdef ?f (getCmdLoc ?c) = Some (insn_cmd ?c) =>
+  eapply IngetCmdsIDs__lookupCmdViaIDFromFdef; 
+    eauto 1 using in_middle
+end.
+
+Ltac repeat_solve :=
+  repeat (match goal with
+          | |- _ => split; eauto 2 using cmds_at_block_tail_next
+          end).
+
+Lemma die_is_sim_removable_state: forall (diinfo : DIInfo) 
+  (Cfg1 : OpsemAux.Config) (St1 : Opsem.State) (Cfg2 : OpsemAux.Config)
+  (St2 : Opsem.State) (Hwfpp : OpsemPP.wf_State Cfg1 St1)
+  (Hsim : State_simulation diinfo Cfg1 St1 Cfg2 St2)
+  (Hrem : removable_State diinfo St1) (Hwfcfg: OpsemPP.wf_Config Cfg1)
+  (St1' : Opsem.State) (tr1 : trace)
+  (Hop1 : Opsem.sInsn Cfg1 St1 St1' tr1),
+  State_simulation diinfo Cfg1 St1' Cfg2 St2 /\ tr1 = E0.
+Proof.
+  intros. 
+  apply removable_State_inv' in Hrem.
+  destruct Hrem as [F1 [b1 [c1 [cs1 [tmn1 [lc1 [als1 [ECs1 [M1 
+     [EQ1 [EQ2 Hdid]]]]]]]]]]]; subst.
+  destruct Cfg1 as [S1 TD1 Ps1 gl1 fs1].
+  destruct_ctx_other.
+  assert (pure_cmd (insn_cmd c1)) as Hpure.
+    apply (DI_pure diinfo); auto.
+      eapply wf_system__uniqFdef in HFinPs1; eauto 1.
+      rewrite Hdid.
+      solve_lookupCmdViaIDFromFdef.
+  inv Hop1; tinv Hpure;
+    abstract (
+      simpl in Hdid; subst;
+      eapply RemoveSim.cmds_simulation_elim_cons_inv in Hcssim2; eauto;
+       repeat_solve; try solve [
+         eauto 2 using cmds_at_block_tail_next,
+                       reg_simulation_update_dead |
+         destruct_if; eauto using reg_simulation_update_dead
+       ]
+    ).
+Qed.
+
+Ltac value_doesnt_use_did_tac :=
+match goal with
+| |- value_doesnt_use_did ?diinfo _ _ =>
+  try solve [
+    eapply conditional_used_in_fdef__used_in_tmn_value; 
+      destruct diinfo; eauto; simpl; auto |
+    eapply conditional_used_in_fdef__used_in_cmd_value; 
+      destruct diinfo; eauto 1 using in_middle; simpl; auto
+  ]
+| |- DI_f ?diinfo <> _ \/
+     fold_left
+       (fun (re : bool) (p : phinode) => re || used_in_phi (DI_id ?diinfo) p)
+       _ false = false =>
+  eapply conditional_used_in_fdef__used_in_phis; destruct diinfo; eauto
+| |- list_value_doesnt_use_did ?diinfo _ _ =>
+    eapply conditional_used_in_fdef__used_in_list_value; 
+      destruct diinfo; eauto using in_middle; simpl; auto
+end.  
+
+Lemma simulation__values2GVs : forall lc lc2 los nts gl F idxs 
+  dinfo (Hprop: list_value_doesnt_use_did dinfo F idxs),
+  reg_simulation dinfo F lc lc2 ->
+  Opsem.values2GVs (los,nts) idxs lc gl = Opsem.values2GVs (los,nts) idxs lc2 gl.
+Proof.
+  induction idxs as [|[]]; simpl; intros.
+    auto.
+
+    inv_mbind'. symmetry_ctx.
+    assert (list_value_doesnt_use_did dinfo F idxs /\
+            value_doesnt_use_did dinfo F v) as J.
+      unfold list_value_doesnt_use_did in *.
+      unfold value_doesnt_use_did in *.
+      simpl in Hprop.
+      destruct Hprop as [Hprop | Hprop]; auto.
+      apply orb_false_iff in Hprop.
+      destruct Hprop; auto.
+    destruct J as [J1 J2].
+    erewrite simulation__getOperandValue; eauto.
+    erewrite IHidxs; eauto.
+Qed.
+
+Ltac simulation__getOperandValue_tac :=
+match goal with
+| Hrsim: reg_simulation  _ _ ?lc1 ?lc2,
+  H1 : Opsem.values2GVs _ ?idxs ?lc1 _ = ret _,
+  H2 : Opsem.values2GVs _ ?idxs ?lc2 _= ret _ |- _ =>
+    erewrite simulation__values2GVs in H1; try solve [
+      eauto 2 | value_doesnt_use_did_tac
+    ];
+    rewrite H1 in H2; inv H2; clear H1
+| Hrsim: reg_simulation  _ _ ?lc1 ?lc2,
+  H1 : Opsem.getOperandValue _ ?v ?lc1 _ = ret _,
+  H2 : Opsem.getOperandValue _ ?v ?lc2 _ = ret _ |- _ =>
+    erewrite simulation__getOperandValue in H1; try solve [
+      eauto 2 | value_doesnt_use_did_tac
+    ];
+    rewrite H1 in H2; inv H2; clear H1
+end.
+
+Ltac die_is_sim_branch := 
+  let foo diinfo b1 b2 f1 f2 :=
+    assert (block_simulation diinfo f1 b1 b2) as Hbsim; try solve[
+      try simulation__getOperandValue_tac;
+      try destruct_if; eapply RemoveSim.fdef_sim__block_sim; eauto
+    ];
+    assert (Hbsim':=Hbsim);
+    apply RemoveSim.block_simulation_inv in Hbsim';
+    destruct Hbsim' as [Heq1 [Hpssim' [Hcssim' Heq5]]]; subst;
+    assert (uniqFdef f1) as Huniq; try solve [eauto using wf_system__uniqFdef]
+  in
+
+  destruct_ctx_other;
+  match goal with
+  | Hcssim2: cmds_simulation _ _ nil _,
+    Hop2: Opsem.sInsn _ _ _ _ |- _ =>
+    apply RemoveSim.cmds_simulation_nil_inv in Hcssim2; subst;
+    inv Hop2;
+    uniq_result
+  end;
+
+  match goal with
+  | H1: Some ?b1 = (if _ then lookupBlockViaLabelFromFdef ?f1 _ else _),
+    H2: Some ?b2 = (if _ then lookupBlockViaLabelFromFdef ?f2 _ else _),
+    Hfsim: fdef_simulation ?diinfo ?f1 ?f2
+   |- _ => foo diinfo b1 b2 f1 f2
+  | H1: Some ?b1 = lookupBlockViaLabelFromFdef ?f1 _,
+    H2: Some ?b2 = lookupBlockViaLabelFromFdef ?f2 _,
+    Hfsim: fdef_simulation ?diinfo ?f1 ?f2
+   |- _ => foo diinfo b1 b2 f1 f2
+  end;
+
+  match goal with
+  | Hfsim: fdef_simulation ?diinfo ?f1 ?f2,
+    Hbsim: block_simulation ?diinfo ?f1 ?b1 ?b2,
+    Hbsim2: block_simulation ?diinfo ?f1 ?b1' ?b2',
+    Hpssim': RemoveSim.phis_simulation _ _ ?f1 _ _,
+    _: Opsem.switchToNewBasicBlock _ ?b1 ?b1' _ _ = Some ?lc1',
+    _: Opsem.switchToNewBasicBlock _ ?b2 ?b2' _ _ = Some ?lc2'
+   |- _ =>
+    assert (blockInFdefB b1 f1) as HBinF1'; try solve_blockInFdefB;
+    eapply phis_simulation_inv in Hpssim'; eauto 2;
+    subst;
+    assert (reg_simulation diinfo f1 lc1' lc2') as Hlcsim2'; try solve [
+      assert (HBinF1'':=HBinF1');
+      eapply wf_system__blockInFdefB__wf_block in HBinF1''; eauto;
+      inv HBinF1'';
+      eapply switchToNewBasicBlock_rsim in Hbsim2;
+        eauto 1; value_doesnt_use_did_tac
+    ];
+    repeat_solve;
+    match goal with
+    | |- exists _:_, exists _:_, exists _:_,
+         block_intro ?l'0 ?ps'0 ?cs' ?tmn'0 =
+         block_intro _ _ (_ ++ ?cs') ?tmn'0 =>
+      exists l'0; exists ps'0; exists nil; auto
+    end
+  end.
+
+Ltac die_is_sim_common_case :=
+match goal with
+| Hcssim2: cmds_simulation _ _ (_::_) _,
+  Hop2: Opsem.sInsn _ _ _ _ |- _ =>
+  apply RemoveSim.cmds_simulation_nelim_cons_inv in Hcssim2; simpl; auto;
+  destruct Hcssim2 as [cs3' [Heq Hcssim2]]; subst;
+  inv Hop2; uniq_result;
+  unfold Opsem.BOP, Opsem.FBOP, Opsem.TRUNC, Opsem.EXT, Opsem.CAST,
+    Opsem.ICMP, Opsem.FCMP, Opsem.GEP in *; 
+  inv_mbind; symmetry_ctx;
+  repeat simulation__getOperandValue_tac; uniq_result;
+  repeat_solve; try solve [
+    try destruct_if;
+    apply reg_simulation_update; auto
+  ]
+end.
+
 Lemma die_is_sim : forall diinfo Cfg1 St1 Cfg2 St2
-  (Hwfpp: OpsemPP.wf_State Cfg1 St1)
+  (Hwfpp: OpsemPP.wf_State Cfg1 St1) (Hwfcfg: OpsemPP.wf_Config Cfg1)
   (Hsim: State_simulation diinfo Cfg1 St1 Cfg2 St2),
   (forall (Hrem: removable_State diinfo St1) St1' tr1
      (Hop1: Opsem.sInsn Cfg1 St1 St1' tr1),
@@ -470,8 +729,8 @@ Local Opaque inscope_of_tmn inscope_of_cmd.
 
   intros.
   split; intros.
-(*
-Case "removable state". eapply dae_is_sim_removable_state; eauto.
+
+Case "removable state". eapply die_is_sim_removable_state; eauto.
 
 Case "unremovable state".
   apply RemoveSim.not_removable_State_inv in Hnrem.
@@ -481,247 +740,56 @@ SCase "sReturn".
 Focus.
 
   destruct_ctx_return.
-  assert (PI_f pinfo <> F' \/ PI_id pinfo <> getCmdLoc (insn_call i0 n c t0 v0 v p))
+  assert (DI_f diinfo <> F' \/ 
+          DI_id diinfo <> getCmdLoc (insn_call i0 n c t0 v0 v p))
     as Hneq.
-    WF_PhiInfo_spec10_tac.
+    destruct Heq3' as [l1 [ps1 [cs11 Heq3']]]; subst.
+    eapply dont_remove_impure_cmd; eauto 2 using in_middle, wf_system__uniqFdef.
   apply RemoveSim.cmds_simulation_nelim_cons_inv in Hcssim2'; auto.
   destruct Hcssim2' as [cs3' [Heq Hcssim2']]; subst;
   inv Hop2;
   uniq_result.
-  eapply free_allocas_return_sim in Hmsim; eauto.
-  exists mi.
   repeat_solve.
-    eapply returnUpdateLocals_als_simulation; eauto.
-
     eapply returnUpdateLocals_reg_simulation with (lc:=lc);
-      eauto using mem_simulation__wf_sb_sim;
-      try solve [get_wf_value_for_simop'; eauto].
-      eapply conditional_used_in_fdef__used_in_tmn_value; eauto; simpl; auto.
+      eauto 1.
+      value_doesnt_use_did_tac.
 
 Unfocus.
 
 SCase "sReturnVoid".
 Focus.
   destruct_ctx_return.
-  assert (PI_f pinfo <> F' \/ PI_id pinfo <> getCmdLoc (insn_call i0 n c t0 v0 v p))
+  assert (DI_f diinfo <> F' \/ 
+          DI_id diinfo <> getCmdLoc (insn_call i0 n c t0 v0 v p))
     as Hneq.
-    WF_PhiInfo_spec10_tac.
+    destruct Heq3' as [l1 [ps1 [cs11 Heq3']]]; subst.
+    eapply dont_remove_impure_cmd; eauto 2 using in_middle, wf_system__uniqFdef.
   apply RemoveSim.cmds_simulation_nelim_cons_inv in Hcssim2'; auto.
   destruct Hcssim2' as [cs3' [Heq Hcssim2']]; subst;
   inv Hop2;
   uniq_result.
-  eapply free_allocas_return_void_sim in Hmsim; eauto.
-  exists mi.
   repeat_solve.
 
 Unfocus.
 
-SCase "sBranch".
-Focus.
-  destruct_ctx_other.
-  apply RemoveSim.cmds_simulation_nil_inv in Hcssim2; subst.
-  inv Hop2.
-  uniq_result.
-
-  assert (block_simulation pinfo F (block_intro l' ps' cs' tmn')
-           (block_intro l'0 ps'0 cs'0 tmn'0)) as Hbsim.
-    destruct Hmsim as [_ [_ Hwf_mi]].
-    eapply simulation__getOperandValue in Hlcsim2;
-      try solve [get_wf_value_for_simop'; eauto 2].
-      erewrite simulation__isGVZero in H1; eauto.
-      clear - H22 H1 Hfsim2.
-      destruct (isGVZero (los, nts) c0); 
-        eapply RemoveSim.fdef_sim__block_sim; eauto.
-
-      eapply conditional_used_in_fdef__used_in_tmn_value; eauto; simpl; auto.
-
-  assert (Hbsim':=Hbsim).
-  apply RemoveSim.block_simulation_inv in Hbsim'.
-  destruct Hbsim' as [Heq1 [Hpssim' [Hcssim' Heq5]]]; subst.
-
-  assert (uniqFdef F) as Huniq. eauto using wf_system__uniqFdef.
-  assert (blockInFdefB (block_intro l'0 ps' cs' tmn'0) F) as HBinF1'.
-    solve_blockInFdefB.
-  eapply phis_simulation_inv in Hpssim'; eauto 2.
-  subst.
-
-  assert (reg_simulation pinfo mi F lc' lc'0) as Hlcsim2'.
-    assert (HBinF1'':=HBinF1').
-    eapply wf_system__blockInFdefB__wf_block in HBinF1''; eauto.     
-    inv HBinF1''.
-    eapply switchToNewBasicBlock_rsim in Hbsim2;
-      eauto using mem_simulation__wf_sb_sim, conditional_used_in_fdef__used_in_phis.
-  assert (als_simulation pinfo mi F lc' als als2) as Halsim2'.
-    eapply switchToNewBasicBlock_asim; eauto.
-  exists mi.
-  repeat_solve.
-    exists l'0. exists ps'0. exists nil. auto.
-    exists l'0. exists ps'0. exists nil. auto.
-
-    destruct Hmsim as [J1 [J2 J3]].
-    split; auto.
-    split; auto.
-      intros blk J.
-      apply J2.
-      intro J4. apply J.
-      simpl.
-      eapply switchToNewBasicBlock_isnt_alloca_in_ECs; eauto; simpl; eauto.
-Unfocus.
-
-SCase "sBranch_uncond".
-Focus.
-  destruct_ctx_other.
-  apply RemoveSim.cmds_simulation_nil_inv in Hcssim2; subst.
-  inv Hop2.
-  uniq_result.
-
-  assert (block_simulation pinfo F (block_intro l' ps' cs' tmn')
-           (block_intro l'0 ps'0 cs'0 tmn'0)) as Hbsim.
-    eapply RemoveSim.fdef_sim__block_sim; eauto.
-  assert (Hbsim':=Hbsim).
-  apply RemoveSim.block_simulation_inv in Hbsim'.
-  destruct Hbsim' as [Heq1 [Hpssim' [Hcssim' Heq5]]]; subst.
-
-  assert (uniqFdef F) as Huniq. eauto using wf_system__uniqFdef.
-  assert (blockInFdefB (block_intro l'0 ps' cs' tmn'0) F) as HBinF1'.
-    solve_blockInFdefB.
-  eapply phis_simulation_inv in Hpssim'; eauto 2.
-  subst.
-
-  assert (reg_simulation pinfo mi F lc' lc'0) as Hlcsim2'.
-    assert (HBinF1'':=HBinF1').
-    eapply wf_system__blockInFdefB__wf_block in HBinF1''; eauto.     
-    inv HBinF1''.
-    eapply switchToNewBasicBlock_rsim in Hbsim2;
-      eauto using mem_simulation__wf_sb_sim, conditional_used_in_fdef__used_in_phis.
-  assert (als_simulation pinfo mi F lc' als als2) as Halsim2'.
-    eapply switchToNewBasicBlock_asim; eauto.
-  exists mi.
-  repeat_solve.
-    exists l'0. exists ps'0. exists nil. auto.
-    exists l'0. exists ps'0. exists nil. auto.
-
-    destruct Hmsim as [J1 [J2 J3]].
-    split; auto.
-    split; auto.
-      intros blk J.
-      apply J2.
-      intro J4. apply J. simpl.
-      eapply switchToNewBasicBlock_isnt_alloca_in_ECs; eauto; simpl; eauto.
-Unfocus.
-
-SCase "sBop". abstract (destruct_ctx_other; dse_is_sim_common_case).
-SCase "sFBop". abstract (destruct_ctx_other; dse_is_sim_common_case).
-SCase "sExtractValue". abstract (destruct_ctx_other; dse_is_sim_common_case).
-SCase "sInsertValue". abstract (destruct_ctx_other; dse_is_sim_common_case).
-SCase "sMalloc".
-  abstract (destruct_ctx_other;
-  apply RemoveSim.cmds_simulation_nelim_cons_inv in Hcssim2; simpl; auto;
-  destruct Hcssim2 as [cs3' [Heq Hcssim2]]; subst;
-  inv Hop2; uniq_result;
-  eapply simulation__getOperandValue with (lc2:=lc2) in H0;
-    try simulation__getOperandValue_tac1;
-  eapply mem_simulation__malloc in Hmsim; eauto 2; simpl in Hmsim;
-  destruct Hmsim as [mi' [Hmsim [Hinc [Hprop1 Hprop2]]]];
-  exists mi';
-  repeat_solve; try solve [
-    eapply als_simulation__malloc; eauto | 
-    eapply reg_simulation__malloc; eauto |
-    eapply inject_incr__preserves__ECs_simulation; 
-      try solve [eauto | eapply malloc__isnt_alloca_in_ECs; eauto] |
-    eapply OpsemAux.inject_incr__preserves__ftable_simulation; eauto
-  ]).
-
-SCase "sFree".
-  abstract (destruct_ctx_other;
-  apply RemoveSim.cmds_simulation_nelim_cons_inv in Hcssim2; auto;
-  destruct Hcssim2 as [cs3' [Heq Hcssim2]]; subst;
-  inv Hop2; uniq_result;
-  eapply simulation__getOperandValue with (lc2:=lc2) in H;
-    try simulation__getOperandValue_tac1;
-  eapply mem_simulation__free in Hmsim; eauto 2;
-  exists mi;
-  repeat_solve).
-
-SCase "sAlloca".
-  abstract (destruct_ctx_other;
-  apply RemoveSim.cmds_simulation_nelim_cons_inv in Hcssim2; simpl; auto;
-  destruct Hcssim2 as [cs3' [Heq Hcssim2]]; subst;
-  inv Hop2; uniq_result;
-  eapply simulation__getOperandValue with (lc2:=lc2) in H0;
-    try simulation__getOperandValue_tac1;
-  eapply mem_simulation__malloc in Hmsim; eauto 2; simpl in Hmsim;
-  destruct Hmsim as [mi' [Hmsim [Hinc [Hprop1 Hprop2]]]];
-  exists mi';
-  repeat_solve; try solve [
-    eapply als_simulation__alloca; eauto | 
-    eapply reg_simulation__malloc; eauto |
-    eapply inject_incr__preserves__ECs_simulation; 
-      try solve [eauto | eapply malloc__isnt_alloca_in_ECs; eauto] |
-    eapply OpsemAux.inject_incr__preserves__ftable_simulation; eauto
-  ]).
-
-SCase "sLoad".
-  abstract (destruct_ctx_other;
-  apply RemoveSim.cmds_simulation_nelim_cons_inv in Hcssim2; simpl; auto;
-  destruct Hcssim2 as [cs3' [Heq Hcssim2]]; subst;
-  inv Hop2; uniq_result;
-  exists mi;
-  repeat_solve; try solve [
-    apply als_simulation_update_lc; auto |
-    apply reg_simulation_update_non_palloca; try solve [
-      auto |
-      eapply simulation__mload; try solve [
-        eauto 2 using mem_simulation__wf_sb_sim |
-        simulation__getOperandValue_tac2
-      ]
-    ] |
-    eapply mem_simulation__update_non_palloca; eauto; simpl; eauto
-  ]).
-
-SCase "sStore".
-  abstract (destruct_ctx_other;
-  apply RemoveSim.cmds_simulation_nelim_cons_inv in Hcssim2; auto;
-  destruct Hcssim2 as [cs3' [Heq Hcssim2]]; subst;
-  inv Hop2; uniq_result;
-  exists mi;
-  repeat_solve; try solve [
-    simpl; eapply simulation__mstore; try solve [
-      eauto 2 using mem_simulation__wf_sb_sim |
-      eapply simulation__getOperandValue; eauto using mem_simulation__wf_sb_sim;
-        try solve [eapply conditional_used_in_fdef__used_in_cmd_value;
-                     eauto using in_middle; simpl; auto |
-                   get_wf_value_for_simop; eauto]
-    ]
-  ]).
-
-SCase "sGEP". abstract (destruct_ctx_other; dse_is_sim_common_case).
-SCase "sTrunc". abstract (destruct_ctx_other; dse_is_sim_common_case).
-SCase "sExt". abstract (destruct_ctx_other; dse_is_sim_common_case).
-SCase "sCast". abstract (destruct_ctx_other; dse_is_sim_common_case).
-SCase "sIcmp". abstract (destruct_ctx_other; dse_is_sim_common_case).
-SCase "sFcmp". abstract (destruct_ctx_other; dse_is_sim_common_case).
-SCase "sSelect".
-  destruct_ctx_other.
-  apply RemoveSim.cmds_simulation_nelim_cons_inv in Hcssim2; simpl; auto;
-  destruct Hcssim2 as [cs3' [Heq Hcssim2]]; subst;
-  inv Hop2; uniq_result.
-  exists mi.
-  repeat_solve.
-    destruct (isGVZero (los,nts) c);
-      apply als_simulation_update_lc; auto.
-    erewrite simulation__isGVZero with (c':=c0);
-      simulation__getOperandValue_tac2.
-    destruct (isGVZero (los,nts) c0);
-      apply reg_simulation_update_non_palloca; eauto; try solve [
-        eapply simulation__getOperandValue;
-        eauto using mem_simulation__wf_sb_sim;
-        try solve [eapply conditional_used_in_fdef__used_in_cmd_value;
-                     eauto using in_middle; simpl; auto|
-                   get_wf_value_for_simop; eauto]
-      ].
-    destruct (isGVZero (los,nts) c);
-      eapply mem_simulation__update_non_palloca; eauto; simpl; eauto.
+SCase "sBranch". abstract die_is_sim_branch.
+SCase "sBranch_uncond". abstract die_is_sim_branch.
+SCase "sBop". abstract (destruct_ctx_other; die_is_sim_common_case).
+SCase "sFBop". abstract (destruct_ctx_other; die_is_sim_common_case).
+SCase "sExtractValue". abstract (destruct_ctx_other; die_is_sim_common_case).
+SCase "sInsertValue". abstract (destruct_ctx_other; die_is_sim_common_case).
+SCase "sMalloc". abstract (destruct_ctx_other; die_is_sim_common_case).
+SCase "sFree". abstract (destruct_ctx_other; die_is_sim_common_case).
+SCase "sAlloca". abstract (destruct_ctx_other; die_is_sim_common_case).
+SCase "sLoad". abstract (destruct_ctx_other; die_is_sim_common_case).
+SCase "sStore". abstract (destruct_ctx_other; die_is_sim_common_case).
+SCase "sGEP". abstract (destruct_ctx_other; die_is_sim_common_case).
+SCase "sTrunc". abstract (destruct_ctx_other; die_is_sim_common_case).
+SCase "sExt". abstract (destruct_ctx_other; die_is_sim_common_case).
+SCase "sCast". abstract (destruct_ctx_other; die_is_sim_common_case).
+SCase "sIcmp". abstract (destruct_ctx_other; die_is_sim_common_case).
+SCase "sFcmp". abstract (destruct_ctx_other; die_is_sim_common_case).
+SCase "sSelect". abstract (destruct_ctx_other; die_is_sim_common_case).
 
 SCase "sCall".
   destruct_ctx_other.
@@ -731,29 +799,21 @@ SCase "sCall".
   inv Hop2; uniq_result.
   SSCase "SCall".
 
-  assert (gv_inject mi fptr fptr0) as Hfptr_sim.
-    assert (exists t, wf_value S (module_intro los nts Ps) F fv t) as G.
-      assert (HBinF1':=HBinF1).
-      eapply wf_system__wf_cmd in HBinF1'; eauto using in_middle.     
-      inv HBinF1'. eauto.
-    destruct G.
-    simulation__getOperandValue_tac2.
-
+  simulation__getOperandValue_tac.
   assert (Hfsim1:=Hpsim).
-  eapply TopSim.lookupFdefViaPtr_inj__simulation in Hfsim1; eauto. 
+  eapply TopSim.lookupFdefViaPtr__simulation in Hfsim1; eauto. 
   simpl in Hfsim1.
   assert (Hbsim1:=Hfsim1).
   eapply RemoveSim.fdef_simulation__entry_block_simulation in Hbsim1; eauto.
   assert (Hbsim1':=Hbsim1).
   apply RemoveSim.block_simulation_inv in Hbsim1'.
   destruct Hbsim1' as [Heq' [Hpsim1' [Hcsim1' Htsim1']]]; subst.
-  exists mi.
-    match goal with
-    | H1: OpsemAux.lookupFdefViaPtr _ _ _ = Some ?F,
-      _ : fdef_simulation _ ?F _ |- _ =>
-      apply OpsemAux.lookupFdefViaPtr_inv in H1;
-      eapply wf_system__uniqFdef in H1; eauto 2
-    end.
+  match goal with
+  | H1: OpsemAux.lookupFdefViaPtr _ _ _ = Some ?F,
+    _ : fdef_simulation _ ?F _ |- _ =>
+    apply OpsemAux.lookupFdefViaPtr_inv in H1;
+    eapply wf_system__uniqFdef in H1; eauto 2
+  end.
   repeat_solve.
     exists l'0. exists ps'. exists nil. auto.
     exists l'0. exists ps'0. exists nil. auto.
@@ -761,40 +821,20 @@ SCase "sCall".
     apply RemoveSim.fdef_simulation_inv in Hfsim1.
     destruct Hfsim1 as [Hfhsim1 Hbssim1].
     inv Hfhsim1.
-    assert (HBinF1':=HBinF1).
-    eapply wf_system__wf_cmd in HBinF1'; eauto using in_middle.     
-    inv HBinF1'.
-    find_wf_value_list.  
     eapply reg_simulation__initLocals; try solve [
-      eauto 2 using mem_simulation__wf_sb_sim, WF_PhiInfo__args_dont_use_pid |
-      eapply conditional_used_in_fdef__used_in_params; eauto 1
+      eauto 2 |
+      eapply conditional_used_in_fdef__used_in_params; destruct diinfo; eauto 1
     ].
-
-    destruct Hmsim as [Hmsim1 [Hmsim2 Hmsim3]].
-    split; auto.
-    split; auto.
-      intros blk J.
-      apply Hmsim2.
-      intro G. apply J.
-      unfold isnt_alloca_in_ECs in *.
-      intros. simpl in Hin.
-      destruct Hin as [Hin | Hin].
-        subst. simpl.
-        inv Hin. eapply WF_PhiInfo__isnt_alloca_in_EC; eauto.
-
-        apply G. simpl. auto.
 
   SSCase "sExCall".
 
-  assert (gv_inject mi fptr fptr0) as Hfptr_sim.
-    assert (exists t, wf_value S (module_intro los nts Ps) F fv t) as G.
-      assert (HBinF1':=HBinF1).
-      eapply wf_system__wf_cmd in HBinF1'; eauto using in_middle.     
-      inv HBinF1'. eauto.
-    destruct G.
-    simulation__getOperandValue_tac2.
-
-  eapply TopSim.lookupFdefViaPtr_inj__simulation_l2r in H1; eauto.
+  simulation__getOperandValue_tac.
+  eapply TopSim.lookupFdefViaPtr__simulation_l2r in H1; eauto.
+  destruct H1 as [f2 [H1 H2']].
+  apply OpsemAux.lookupExFdecViaPtr_inversion in H29.
+  apply OpsemAux.lookupFdefViaPtr_inversion in H1.
+  destruct H29 as [fn [J1 [J2 J3]]].
+  destruct H1 as [fn' [J4 J5]].
   uniq_result.
 
 SCase "sExCall".
@@ -807,248 +847,42 @@ SCase "sExCall".
 
   SSCase "SCall".
 
-  assert (gv_inject mi fptr fptr0) as Hfptr_sim.
-    assert (exists t, wf_value S (module_intro los nts Ps) F fv t) as G.
-      assert (HBinF1':=HBinF1).
-      eapply wf_system__wf_cmd in HBinF1'; eauto using in_middle.     
-      inv HBinF1'. eauto.
-    destruct G.
-    simulation__getOperandValue_tac2.
-
-  eapply TopSim.lookupFdefViaPtr_inj__simulation_r2l in H1; eauto.
+  simulation__getOperandValue_tac.
+  match goal with
+  | Hpsim: products_simulation _ ?Ps ?Ps2,
+    H1: OpsemAux.lookupExFdecViaPtr ?Ps _ _ = _,
+    H30: OpsemAux.lookupFdefViaPtr ?Ps2 _ _ = _ |- _ =>
+    clear - H30 H1 Hpsim;
+    eapply TopSim.lookupExFdecViaPtr__simulation_l2r in H1; eauto;
+    simpl in H1;
+    apply OpsemAux.lookupExFdecViaPtr_inversion in H1;
+    apply OpsemAux.lookupFdefViaPtr_inversion in H30;
+    destruct H1 as [fn [J1 [J2 J3]]];
+    destruct H30 as [fn' [J4 J5]]
+  end.
   uniq_result.
 
   SSCase "sExCall".
 
-  assert (gv_inject mi fptr fptr0) as Hfptr_sim.
-    assert (exists t, wf_value S (module_intro los nts Ps) F fv t) as G.
-      assert (HBinF1':=HBinF1).
-      eapply wf_system__wf_cmd in HBinF1'; eauto using in_middle.     
-      inv HBinF1'. eauto.
-    destruct G.
-    simulation__getOperandValue_tac2.
+  simulation__getOperandValue_tac.
+  assert (Hlkdec:=Hpsim).
+  eapply TopSim.lookupExFdecViaPtr__simulation_l2r in Hlkdec; eauto.
 
-  eapply TopSim.lookupExFdecViaPtr_inj__simulation in Hfptr_sim; eauto.
+  assert (gvss = gvss0) as EQ.
+    inv_mfalse; symmetry_ctx.
+    erewrite reg_simulation__params2GVs in H2; eauto.
+      uniq_result. auto.
+      eapply conditional_used_in_fdef__used_in_params; destruct diinfo; eauto 1.
+  subst.
   uniq_result.
-
-  match goal with | H1 : fdec_intro _ _ = fdec_intro _ _ |- _ => inv H1 end.
-  assert (List.Forall2 (fun gv1 => fun gv2 => gv_inject mi gv1 gv2) gvss gvss0)
-    as Hparsim.
-    assert (HBinF1':=HBinF1).
-    eapply wf_system__wf_cmd in HBinF1'; eauto using in_middle.     
-    inv HBinF1'.
-    find_wf_value_list.  
-    eapply reg_simulation__params2GVs; try solve [
-      eauto 2 using mem_simulation__wf_sb_sim |
-      eapply conditional_used_in_fdef__used_in_params; eauto 1
-    ].
-  eapply callExternalFunction__mem_simulation in Hmsim; eauto.
-  destruct Hmsim as [EQ' [EQ [mi' [Hmsim [Hinc [J1 [J2 J3]]]]]]]; subst.
-  exists mi'.
   repeat_solve.
-    eapply inject_incr__preserves__ECs_simulation; eauto.
-    eapply OpsemAux.inject_incr__preserves__ftable_simulation; eauto.
+    eapply exCallUpdateLocals_reg_simulation; eauto.
 
 Transparent inscope_of_tmn inscope_of_cmd.
 
 Qed.
+(* The reg_simulation_update_non_palloca in dae_defs.v may not use to check
+   if the updated id is dead or not, refer to the reg_simulation_update in this
+   proof. Other lemmas that use it could be simplified too.
 *)
-Admitted.
-
-Lemma s_genInitState__die_State_simulation:
-  forall diinfo S1 S2 main VarArgs cfg2 IS2,
-  system_simulation diinfo S1 S2 ->
-  Opsem.s_genInitState S2 main VarArgs Mem.empty = ret (cfg2, IS2) ->
-  exists cfg1, exists IS1,
-    Opsem.s_genInitState S1 main VarArgs Mem.empty = ret (cfg1, IS1) /\
-    State_simulation diinfo cfg1 IS1 cfg2 IS2.
-Admitted.
-
-Lemma s_isFinialState__die_State_simulation_l2r:
-  forall diinfo cfg1 FS1 cfg2 FS2 r
-  (Hstsim : State_simulation diinfo cfg1 FS1 cfg2 FS2)
-  (Hfinal: Opsem.s_isFinialState cfg1 FS1 = ret r),
-  Opsem.s_isFinialState cfg2 FS2 = ret r.
-Admitted.
-
-Lemma s_isFinialState__die_State_simulation_l2r':
-  forall diinfo cfg1 FS1 cfg2 FS2
-  (Hstsim : State_simulation diinfo cfg1 FS1 cfg2 FS2)
-  (Hfinal: Opsem.s_isFinialState cfg1 FS1 <> None),
-  Opsem.s_isFinialState cfg2 FS2 <> None.
-Admitted.
-
-Lemma s_isFinialState__die_State_simulation_r2l:
-  forall diinfo cfg1 FS1 cfg2 FS2 r
-  (Hstsim : State_simulation diinfo cfg1 FS1 cfg2 FS2)
-  (Hfinal: Opsem.s_isFinialState cfg2 FS2 = ret r),
-  exists FS1', 
-    Opsem.sop_star cfg1 FS1 FS1' E0 /\
-    State_simulation diinfo cfg1 FS1' cfg2 FS2 /\
-    Opsem.s_isFinialState cfg1 FS1' = ret r.
-Admitted.
-
-Lemma s_isFinialState__die_State_simulation_None_r2l:
-  forall diinfo cfg1 FS1 cfg2 FS2
-  (Hstsim : State_simulation diinfo cfg1 FS1 cfg2 FS2)
-  (Hfinal: Opsem.s_isFinialState cfg2 FS2 = None),
-  Opsem.s_isFinialState cfg1 FS1 = None.
-Admitted.
-
-Lemma undefined_state__die_State_simulation_r2l: forall diinfo cfg1 St1 cfg2
-  St2 (Hstsim : State_simulation diinfo cfg1 St1 cfg2 St2),
-  OpsemPP.undefined_state cfg2 St2 -> OpsemPP.undefined_state cfg1 St1.
-Admitted.
-
-Lemma undefined_state__die_State_simulation_l2r: forall diinfo cfg1 St1 cfg2
-  St2 (Hstsim : State_simulation diinfo cfg1 St1 cfg2 St2),
-  OpsemPP.undefined_state cfg1 St1 -> OpsemPP.undefined_state cfg2 St2.
-Admitted.
-
-Lemma sop_star__die_State_simulation: forall diinfo cfg1 IS1 cfg2 IS2 tr FS2 
-  (Hwfcfg: OpsemPP.wf_Config cfg1) (Hwfpp: OpsemPP.wf_State cfg1 IS1) 
-  (Hstsim : State_simulation diinfo cfg1 IS1 cfg2 IS2)
-  (Hopstar : Opsem.sop_star cfg2 IS2 FS2 tr),
-  exists FS1, Opsem.sop_star cfg1 IS1 FS1 tr /\
-    State_simulation diinfo cfg1 FS1 cfg2 FS2.
-Proof.
-  intros.
-  generalize dependent IS1.
-  induction Hopstar; intros.
-    exists IS1. split; auto.
-
-    assert (J:=Hwfpp).
-    apply OpsemPP.progress in J; auto.
-    destruct J as [Hfinal1 | [[IS1' [tr0 Hop1]] | Hundef1]].
-      eapply s_isFinialState__die_State_simulation_l2r' in Hstsim; eauto 1.
-      contradict H; eauto using s_isFinialState__stuck.
-
-      assert (OpsemPP.wf_State cfg1 IS1') as Hwfpp'.
-        apply OpsemPP.preservation in Hop1; auto.
-      eapply die_is_sim in Hstsim; eauto.
-      destruct Hstsim as [Hstsim1 Hstsim2].
-      destruct (@RemoveSim.removable_State_dec 
-          (DI_f diinfo) (DI_id diinfo) IS1) as [Hrm | Hnrm].
-        eapply Hstsim1 in Hrm; eauto.
-        destruct Hrm as [Hstsim EQ]; subst.
-        admit. (* we should do induction on the measure of State_simulation *)
-
-        eapply Hstsim2 in Hnrm; eauto.
-        destruct Hnrm as [Hstsim EQ]; subst.
-        eapply IHHopstar in Hstsim; eauto.
-        destruct Hstsim as [FS1 [Hopstar1 Hstsim]].
-        exists FS1.
-        split; eauto.
-
-      eapply undefined_state__die_State_simulation_l2r in Hstsim; eauto.
-      contradict H; eauto using undefined_state__stuck.
-Qed.
-
-Lemma sop_div__die_State_simulation: forall diinfo cfg1 IS1 cfg2 IS2 tr
-  (Hwfpp: OpsemPP.wf_State cfg1 IS1)
-  (Hstsim : State_simulation diinfo cfg1 IS1 cfg2 IS2)
-  (Hopstar : Opsem.sop_diverges cfg2 IS2 tr),
-  Opsem.sop_diverges cfg1 IS1 tr.
-Admitted.
-
-Lemma die_wfS: forall id0 f diinfo los nts Ps1 Ps2
-  (HwfS: wf_system [module_intro los nts (Ps1 ++ product_fdef f :: Ps2)])
-  (Heq1: f = DI_f diinfo) (Heq2: id0 = DI_id diinfo),
-  wf_system 
-    [module_intro los nts (Ps1 ++  product_fdef (remove_fdef id0 f) :: Ps2)].
-Admitted.
-
-Lemma die_sim: forall id0 f diinfo los nts Ps1 Ps2 main VarArgs
-  (HwfS: wf_system [module_intro los nts (Ps1 ++ product_fdef f :: Ps2)])
-  (Hok: defined_program [module_intro los nts (Ps1 ++ product_fdef f :: Ps2)] 
-          main VarArgs)
-  (Heq1: f = DI_f diinfo) (Heq2: id0 = DI_id diinfo),
-  program_sim
-    [module_intro los nts
-      (Ps1 ++  product_fdef (remove_fdef id0 f) :: Ps2)]
-    [module_intro los nts (Ps1 ++ product_fdef f :: Ps2)]
-    main VarArgs.
-Proof.
-  intros. subst.
-  assert (Huniq:=HwfS). apply wf_system__uniqSystem in Huniq; auto.
-  assert (system_simulation diinfo
-    [module_intro los nts (Ps1 ++ product_fdef (DI_f diinfo) :: Ps2)]
-    [module_intro los nts
-      (Ps1 ++ product_fdef (remove_fdef (DI_id diinfo) (DI_f diinfo)) :: Ps2)])
-    as Hssim.
-    constructor; auto.
-    repeat split; auto.    
-    unfold TopSim.products_simulation. simpl. unfold system_simulation.
-    simpl in Huniq. destruct Huniq as [[_ [_ Huniq]] _].
-    apply uniq_products_simulation; auto.
-
-  constructor; auto.
-    intros tr t Hconv.
-    inv Hconv.
-    eapply s_genInitState__die_State_simulation in H; eauto.
-    destruct H as [cfg1 [IS1 [Hinit1 Hstsim]]].    
-    assert (OpsemPP.wf_Config cfg1 /\ OpsemPP.wf_State cfg1 IS1) as Hwfst. 
-      eapply s_genInitState__opsem_wf; eauto.
-    eapply sop_star__die_State_simulation in Hstsim; eauto; try tauto.
-    destruct Hstsim as [FS1 [Hopstar1 Hstsim']].
-    eapply s_isFinialState__die_State_simulation_r2l in Hstsim'; eauto.
-    destruct Hstsim' as [FS1' [Hopstar1' [Hstsim'' Hfinal]]].
-    assert (Opsem.sop_star cfg1 IS1 FS1' tr) as Hopstar1''.
-      rewrite <- E0_right.
-      eapply OpsemProps.sop_star_trans; eauto.
-    exists t. split; auto using result_match_relf. econstructor; eauto.
-
-    intros tr Hdiv.
-    inv Hdiv.
-    eapply s_genInitState__die_State_simulation in H; eauto.
-    destruct H as [cfg1 [IS1 [Hinit Hstsim]]].
-    assert (OpsemPP.wf_State cfg1 IS1) as Hwfst.
-      eapply s_genInitState__opsem_wf; eauto.
-    eapply sop_div__die_State_simulation in Hstsim; eauto.
-    destruct Hstsim as [FS1 Hopdiv1].
-    econstructor; eauto.
-
-    intros tr t Hgowrong.
-    inv Hgowrong.
-    assert (OpsemPP.wf_Config cfg /\ OpsemPP.wf_State cfg t) as HwfSt.
-      eapply s_genInitState__opsem_wf in H; eauto using die_wfS.
-      destruct H as [Hcfg2 HwfSt2].
-      apply OpsemPP.preservation_star in H0; auto.
-    assert (OpsemPP.undefined_state cfg t) as Hundef.
-      apply stuck__undefined_state in H2; try solve [auto | tauto].
-    eapply s_genInitState__die_State_simulation in H; eauto.
-    destruct H as [cfg1 [IS1 [Hinit Hstsim]]].
-    assert (OpsemPP.wf_Config cfg1 /\ OpsemPP.wf_State cfg1 IS1) as Hwfst. 
-      eapply s_genInitState__opsem_wf; eauto.
-    eapply sop_star__die_State_simulation in Hstsim; eauto; try tauto.
-    destruct Hstsim as [FS1 [Hopstar1 Hstsim']].
-    assert (OpsemPP.undefined_state cfg1 FS1) as Hundef'.
-      eapply undefined_state__die_State_simulation_r2l in Hundef; 
-        try solve [eauto | tauto].
-    assert (Opsem.s_isFinialState cfg1 FS1 = merror) as Hfinal'.
-      eapply s_isFinialState__die_State_simulation_None_r2l in H2; 
-        try solve [eauto | tauto].
-    apply undefined_state__stuck' in Hundef'.
-    exists tr. exists FS1.
-    econstructor; eauto.
-Qed.
-
-Lemma subst_fdef__diinfo: forall f id0 v0,
-  exists diinfo:DIInfo, DI_f diinfo = subst_fdef id0 v0 f /\ DI_id diinfo = id0.
-Admitted.
-
-Lemma die_wfPI: forall id0 f diinfo los nts Ps1 Ps2 pinfo
-  (Hwfpi: WF_PhiInfo pinfo)
-  (HwfS: wf_system [module_intro los nts (Ps1 ++ product_fdef f :: Ps2)])
-  (Heq1: f = DI_f diinfo) (Heq2: id0 = DI_id diinfo) (Heq3: f = PI_f pinfo),
-  WF_PhiInfo (update_pinfo pinfo (remove_fdef id0 f)).
-Admitted.
-
-Lemma remove_successors : forall f id',
-  successors f = successors (remove_fdef id' f).
-Admitted.
-
-Lemma remove_reachablity_analysis : forall f id',
-  reachablity_analysis f = reachablity_analysis (remove_fdef id' f).
-Admitted.
 
