src3.0/Transforms/die_top.v
@@ -1,0 +1,885 @@
+Require Import vellvm.
+Require Import Kildall.
+Require Import ListSet.
+Require Import Maps.
+Require Import Lattice.
+Require Import Iteration.
+Require Import Maps.
+Require Import opsem_props.
+Require Import primitives.
+Require Import memory_sim.
+Require Import memory_props.
+Require Import program_sim.
+Require Import palloca_props.
+Require Import top_sim.
+Require Import trans_tactic.
+Require Import die.
+Require Import die_wfS.
+
+Lemma s_genInitState__die_State_simulation':
+  forall diinfo S1 S2 main VarArgs cfg2 IS2,
+  system_simulation diinfo S1 S2 ->
+  Opsem.s_genInitState S2 main VarArgs Mem.empty = ret (cfg2, IS2) ->
+  exists cfg1, exists IS1,
+    Opsem.s_genInitState S1 main VarArgs Mem.empty = ret (cfg1, IS1) /\
+    State_simulation diinfo cfg1 IS1 cfg2 IS2 /\
+    genericvalues_inject.wf_globals (Mem.nextblock (Opsem.Mem IS1) - 1) 
+      (OpsemAux.Globals cfg1).
+Proof.
+    unfold Opsem.s_genInitState.
+    intros.
+    inv_mbind'.
+    destruct m as [los nts ps].
+    inv_mbind'.
+    destruct b as [l0 ps0 cs0 tmn0].
+    destruct f as [[fa rt fid la va] bs].
+    inv_mbind'. symmetry_ctx.
+    assert (HlkF2FromS2:=HeqR).
+    eapply TopSim.system_simulation__fdef_simulation_r2l in HeqR; eauto.
+    destruct HeqR as [f1 [HlkF1fromS1 Hfsim]]. simpl in Hfsim.
+    fill_ctxhole.
+    eapply TopSim.system_simulation__getParentOfFdefFromSystem in HeqR0; eauto.
+    destruct HeqR0 as [m1 [J1 J2]].
+    fill_ctxhole. destruct m1 as [los1 nts1 ps1].
+    destruct J2 as [J2 [J3 J4]]; subst.
+    eapply TopSim.genGlobalAndInitMem_spec in HeqR1; eauto.
+    destruct HeqR1 as [gl1 [fs1 [M1 [HeqR1 [EQ1 [EQ2 EQ3]]]]]]; subst.
+    fill_ctxhole.
+    assert (J:=HeqR2).
+    eapply RemoveSim.getEntryBlock__simulation in J; eauto.
+    destruct J as [b1 [J5 J6]].
+    fill_ctxhole.
+    destruct b1 as [l2 ps2 cs2 tmn2].
+    destruct f1 as [[fa1 rt1 fid1 la1 va1] bs1].
+    assert (J:=Hfsim).
+    apply RemoveSim.fdef_simulation__eq_fheader in J.
+    inv J.
+    fill_ctxhole. eauto.
+  match goal with
+  | |- exists _:_, exists _:_, Some (?A, ?B) = _ /\ _ => exists A; exists B
+  end.
+  match goal with 
+  | H: getParentOfFdefFromSystem _ _ = _ |- _ =>
+    apply getParentOfFdefFromSystem__moduleInProductsInSystemB in H;
+    destruct H as [HMinS HinPs]
+  end.
+  assert (J:=J6).
+  apply RemoveSim.block_simulation_inv in J.
+  destruct J as [J1 [J2 [J3 J7]]]; subst.
+  assert (blockInFdefB (block_intro l0 ps0 cs0 tmn0)
+           (fdef_intro (fheader_intro fa rt fid la va) bs) = true) as HBinF.
+    apply entryBlockInFdef; auto.
+  split; auto.
+  eapply genGlobalAndInitMem__wf_globals_Mem in HeqR1; eauto.
+  destruct HeqR1 as [J7 [J8 [J9 [J10 [J11 [J12 [J13 J14]]]]]]].
+  repeat (split; auto).
+    exists l0. exists ps2. exists nil. auto.
+    exists l0. exists ps0. exists nil. auto.
+      unfold reg_simulation.
+      destruct_if.
+    simpl.
+    apply MemProps.redundant__wf_globals; auto. 
+    tauto.
+Qed.
+
+Lemma s_genInitState__die_State_simulation:
+  forall diinfo S1 S2 main VarArgs cfg2 IS2
+  (Hstsim: system_simulation diinfo S1 S2)
+  (Hinit: Opsem.s_genInitState S2 main VarArgs Mem.empty = ret (cfg2, IS2)),
+  exists maxb, exists cfg1, exists IS1,
+    Opsem.s_genInitState S1 main VarArgs Mem.empty = ret (cfg1, IS1) /\
+    State_simulation diinfo cfg1 IS1 cfg2 IS2 /\
+    genericvalues_inject.wf_globals maxb (OpsemAux.Globals cfg1) /\
+    0 <= maxb.
+Proof.
+  intros.
+  eapply s_genInitState__die_State_simulation' in Hinit; eauto.
+  destruct Hinit as [cfg1 [IS1 [J1 [J2 J3]]]].
+  exists (Mem.nextblock (Opsem.Mem IS1) - 1).
+  exists cfg1. exists IS1.
+  split; auto.
+  split; auto.
+  split; auto.
+    assert (J:=Mem.nextblock_pos (Opsem.Mem IS1)).
+    omega.
+Qed.
+
+Ltac s_isFinialState__die_State_simulation cfg1 cfg2 FS1 FS2 Hstsim Hfinal := 
+  destruct cfg2 as [S2 [los2 nts2] gl2 fs2];
+  destruct cfg1 as [S1 [los1 nts1] gl1 fs1];
+  destruct FS1 as [[|[? ? cs1 ? ?] ES1]]; 
+  destruct FS2 as [[|[? ? cs2 ? ?] ES2]]; try solve [
+    eauto 3 using result_match_relf |
+    destruct Hstsim as [X [? [Hstsim [? [? ?]]]]]; subst; inv Hstsim
+  ];
+  destruct Hstsim as [X [? [Hstsim [? [? ?]]]]]; subst;
+  inv X; simpl;
+  destruct Hstsim as [Hstsim Hstsim'];
+  fold ECs_simulation in Hstsim';
+  destruct Hstsim as [? [Htmn [? [? [? [? [? Hstsim]]]]]]]; subst;
+  destruct cs1, cs2; try solve [
+    eauto 3 using result_match_relf |
+    apply RemoveSim.cmds_simulation_nil_inv in Hstsim; try congruence |
+    inv Hfinal
+  ].
+
+Lemma s_isFinialState__die_State_simulation_l2r:
+  forall diinfo cfg1 FS1 cfg2 FS2 r1
+  (Hwfcfg2: OpsemPP.wf_Config cfg2) (Hwfpp2: OpsemPP.wf_State cfg2 FS2) 
+  (Hwfcfg1: OpsemPP.wf_Config cfg1) (Hwfpp1: OpsemPP.wf_State cfg1 FS1) 
+  (Hnuse: used_in_fdef (DI_id diinfo) (DI_f diinfo) = false)
+  (Hstsim : State_simulation diinfo cfg1 FS1 cfg2 FS2)
+  (Hfinal: Opsem.s_isFinialState cfg1 FS1 = ret r1),
+  exists r2, Opsem.s_isFinialState cfg2 FS2 = ret r2 /\ result_match r1 r2.
+Proof.
+  unfold Opsem.s_isFinialState.
+  intros.
+  s_isFinialState__die_State_simulation cfg1 cfg2 FS1 FS2 Hstsim Hfinal.
+  destruct Terminator0; eauto 3 using result_match_relf.
+    destruct ES1, ES2; try solve [eauto 3 using result_match_relf | inv Hstsim'].
+      simpl in Hfinal.
+      inTmnOp_isnt_stuck value5 H4 Hwfcfg2 Hwfpp2.
+      destruct H3 as [l5 [ps2 [cs21 H3]]]; subst;
+      destruct Hwfcfg1 as [_ [Hwfg1 [Hwfs1 HmInS1]]];
+      destruct Hwfpp1 as 
+          [_ [[Hreach1 [HbInF1 [HfInPs1 [_ [_ _]]]]] _]].
+      erewrite <- simulation__getOperandValue; eauto.
+      eauto 3 using result_match_relf.
+        value_doesnt_use_did_tac.
+
+    destruct ES1, ES2; try solve [eauto 3 using result_match_relf | inv Hstsim'].
+Qed.
+
+Lemma s_isFinialState__die_State_simulation_l2r':
+  forall diinfo cfg1 FS1 cfg2 FS2 
+  (Hwfcfg2: OpsemPP.wf_Config cfg2) (Hwfpp2: OpsemPP.wf_State cfg2 FS2) 
+  (Hwfcfg1: OpsemPP.wf_Config cfg1) (Hwfpp1: OpsemPP.wf_State cfg1 FS1) 
+  (Hnuse: used_in_fdef (DI_id diinfo) (DI_f diinfo) = false)
+  (Hstsim : State_simulation diinfo cfg1 FS1 cfg2 FS2)
+  (Hfinal: Opsem.s_isFinialState cfg1 FS1 <> None),
+  Opsem.s_isFinialState cfg2 FS2 <> None.
+Proof.
+  intros.
+  remember (Opsem.s_isFinialState cfg1 FS1) as R.
+  destruct R; try congruence.
+  symmetry_ctx.
+  eapply s_isFinialState__die_State_simulation_l2r in Hstsim; eauto.
+  destruct Hstsim as [r2 [Hstim Hinj]].
+  congruence.
+Qed.
+
+Lemma s_isFinialState__die_State_simulation_None_r2l:
+  forall diinfo cfg1 FS1 cfg2 FS2
+  (Hwfcfg2: OpsemPP.wf_Config cfg2) (Hwfpp2: OpsemPP.wf_State cfg2 FS2) 
+  (Hwfcfg1: OpsemPP.wf_Config cfg1) (Hwfpp1: OpsemPP.wf_State cfg1 FS1) 
+  (Hnuse: used_in_fdef (DI_id diinfo) (DI_f diinfo) = false)
+  (Hstsim : State_simulation diinfo cfg1 FS1 cfg2 FS2)
+  (Hfinal: Opsem.s_isFinialState cfg2 FS2 = None),
+  Opsem.s_isFinialState cfg1 FS1 = None.
+Proof.
+  intros.
+  remember (Opsem.s_isFinialState cfg1 FS1) as R.
+  destruct R; try congruence.
+  contradict Hfinal.
+  eapply s_isFinialState__die_State_simulation_l2r' in Hstsim; eauto.
+    congruence.
+Qed.
+
+Lemma s_isFinialState__die_State_simulation_r2l':
+  forall dinfo cfg1 FS1 cfg2 FS2 r2  
+  (Hnuse: used_in_fdef (DI_id dinfo) (DI_f dinfo) = false)
+  (Hwfcfg1: OpsemPP.wf_Config cfg1) (Hwfpp1: OpsemPP.wf_State cfg1 FS1) 
+  (Hstsim : State_simulation dinfo cfg1 FS1 cfg2 FS2)
+  (Hnrem: ~removable_State dinfo FS1) 
+  (Hfinal: Opsem.s_isFinialState cfg2 FS2 = ret r2),
+  exists r1, Opsem.s_isFinialState cfg1 FS1 = ret r1 /\ result_match r1 r2.
+Proof.
+  unfold Opsem.s_isFinialState.
+  intros.
+  s_isFinialState__die_State_simulation cfg1 cfg2 FS1 FS2 Hstsim Hfinal.
+    destruct Terminator0; eauto 3 using result_match_relf.
+      destruct ES1, ES2;try solve [eauto 3 using result_match_relf|inv Hstsim'].
+        simpl in Hfinal.
+        inTmnOp_isnt_stuck value5 H3 Hwfcfg1 Hwfpp1.
+        destruct H3 as [l5 [ps2 [cs21 H3]]]; subst;
+        destruct Hwfcfg1 as [_ [Hwfg1 [Hwfs1 HmInS1]]];
+        destruct Hwfpp1 as 
+          [_ [[Hreach1 [HbInF1 [HfInPs1 [_ [_ _]]]]] _]].
+        erewrite simulation__getOperandValue; eauto.
+        eauto 3 using result_match_relf.
+          value_doesnt_use_did_tac.
+
+      destruct ES1, ES2;try solve [eauto 3 using result_match_relf|inv Hstsim'].
+
+   unfold removable_State in Hnrem.
+   apply RemoveSim.not_removable_State_inv in Hnrem.
+   apply RemoveSim.cmds_simulation_nelim_cons_inv in Hstsim; auto. 
+   destruct Hstsim as [cs2' [J1 Hstsim]]; congruence.
+Qed.
+
+Lemma removable_State__non_removable_State' : forall dinfo f1 b1 c1 cs1 tmn1
+  lc1 als1 ES1 M1 IS1'' tr0 Cfg1
+  (Hex: exists l0, exists ps0, exists cs0, 
+          b1 = block_intro l0 ps0 (cs0 ++ c1 :: cs1) tmn1)
+  (Huniq: uniqFdef f1) (HBinF: blockInFdefB b1 f1 = true)
+  (Hrm : RemoveSim.removable_State (DI_f dinfo) (DI_id dinfo)
+          {|
+          Opsem.ECS := {|
+                       Opsem.CurFunction := f1;
+                       Opsem.CurBB := b1;
+                       Opsem.CurCmds := c1 :: cs1;
+                       Opsem.Terminator := tmn1;
+                       Opsem.Locals := lc1;
+                       Opsem.Allocas := als1 |} :: ES1;
+          Opsem.Mem := M1 |})
+  (Hop1 : Opsem.sInsn Cfg1
+           {|
+           Opsem.ECS := {|
+                        Opsem.CurFunction := f1;
+                        Opsem.CurBB := b1;
+                        Opsem.CurCmds := c1 :: cs1;
+                        Opsem.Terminator := tmn1;
+                        Opsem.Locals := lc1;
+                        Opsem.Allocas := als1 |} :: ES1;
+           Opsem.Mem := M1 |} IS1'' tr0),
+  tr0 = E0 /\ ~ removable_State dinfo IS1''.
+Proof.
+  intros.
+  assert (pure_cmd (insn_cmd c1)) as Hpure.
+    simpl in Hrm.
+    destruct_if.
+    destruct_dec; try tauto.
+    apply (DI_pure dinfo); auto.
+      destruct Hex as [l0 [ps0 [cs0 Hex]]]; subst.
+      rewrite e0.
+      solve_lookupCmdViaIDFromFdef.
+  assert (NoDup (getCmdsLocs (c1 :: cs1))) as Hnodup.
+    destruct Hex as [l0 [ps0 [cs0 Hex]]]; subst.
+    apply uniqFdef__uniqBlockLocs in HBinF; auto.
+    simpl in HBinF. split_NoDup. simpl_locs_in_ctx.
+    split_NoDup. auto.
+  inv Hop1; try solve [
+    inv Hpure |
+    split; try solve
+      [auto | eapply RemoveSim.removable_State__non_removable_State; eauto]
+  ].
+Qed.
+
+Lemma die_is_bsim_removable_steps : forall dinfo Cfg1 St1 Cfg2 St2
+  (Hnuse: used_in_fdef (DI_id dinfo) (DI_f dinfo) = false)
+  (Hwfcfg: OpsemPP.wf_Config Cfg1) (Hwfpp: OpsemPP.wf_State Cfg1 St1)
+  (Hsim: State_simulation dinfo Cfg1 St1 Cfg2 St2)
+  (Hok: ~ sop_goeswrong Cfg1 St1),
+  exists St1',
+    Opsem.sop_star Cfg1 St1 St1' E0 /\
+    State_simulation dinfo Cfg1 St1' Cfg2 St2 /\
+    ~ removable_State dinfo St1'.
+Proof.
+  intros.
+  destruct (@RemoveSim.removable_State_dec (DI_f dinfo) (DI_id dinfo) St1) 
+    as [Hrm | Hnrm]; try solve  [exists St1; split; auto].
+  destruct St1 as [[|[f1 b1 [|c1 cs1] tmn1 lc1 als1] ES1] M1]; tinv Hrm.
+  assert (J:=Hwfpp).
+  apply OpsemPP.progress in J; auto.
+  assert (Hnfinal1:=Hrm).
+  apply RemoveSim.removable_State__isnt__final with (cfg:=Cfg1) in Hnfinal1.
+  destruct J as [Hfinal1 | [[IS1'' [tr0 Hop1]] | Hundef1]]; try congruence.
+    eapply die_is_sim in Hsim; eauto.
+    destruct Hsim as [Hstsim1 _].
+    assert (tr0 = E0 /\ ~ removable_State dinfo IS1'') as Hnrm.
+      apply palloca_props.wf_State__uniqECs in Hwfpp; auto.
+      inv Hwfpp. destruct H1 as [J1 [J2 J3]]. simpl in *.
+      eapply removable_State__non_removable_State' in Hop1; eauto.
+    destruct Hnrm as [EQ Hnrm]; subst.
+    eapply Hstsim1 in Hrm; eauto.
+    destruct Hrm as [Hstsim EQ]; subst.
+    exists IS1''.
+    split; auto. 
+      apply OpsemProps.sInsn__implies__sop_star; auto.
+
+    apply undefined_state__stuck' in Hundef1.
+    contradict Hok. 
+    apply nonfinal_stuck_state_goes_wrong; auto.
+Qed.
+
+Lemma die_is_bsim_unremovable_step : forall dinfo Cfg1 IS1 Cfg2 IS2
+  (Hnuse: used_in_fdef (DI_id dinfo) (DI_f dinfo) = false)
+  (Hok : ~ sop_goeswrong Cfg1 IS1)
+  (Hwfcfg: OpsemPP.wf_Config Cfg1) (Hwfpp: OpsemPP.wf_State Cfg1 IS1)
+  (Hnrm: ~ removable_State dinfo IS1)
+  (Hstsim : State_simulation dinfo Cfg1 IS1 Cfg2 IS2) IS2' tr2
+  (Hop2: Opsem.sInsn Cfg2 IS2 IS2' tr2)
+  (Hwfcfg2: OpsemPP.wf_Config Cfg2) (Hwfpp2: OpsemPP.wf_State Cfg2 IS2),
+  exists IS1' : Opsem.State,
+    Opsem.sInsn Cfg1 IS1 IS1' tr2 /\
+    State_simulation dinfo Cfg1 IS1' Cfg2 IS2'.
+Proof.
+  intros.
+  assert (Hnfinal1: Opsem.s_isFinialState Cfg1 IS1 = merror).
+    remember (Opsem.s_isFinialState Cfg1 IS1) as R.
+    destruct R; auto.
+    apply s_isFinialState__die_State_simulation_l2r' in Hstsim; 
+      try solve [auto | congruence].
+      contradict Hop2; eauto using s_isFinialState__stuck.
+  assert (J:=Hwfpp).
+  apply OpsemPP.progress in J; auto.
+  destruct J as [Hfinal1 | [[IS1'' [tr0 Hop1]] | Hundef1]]; try congruence.
+    assert (OpsemPP.wf_State Cfg1 IS1'') as Hwfpp''.
+      apply OpsemPP.preservation in Hop1; auto.
+    eapply die_is_sim in Hstsim; eauto.
+    destruct Hstsim as [Hstsim1 Hstsim2].
+    eapply Hstsim2 in Hnrm; eauto.
+    destruct Hnrm as [Hstsim EQ]; subst.
+    exists IS1''. 
+    split; eauto.
+
+    apply undefined_state__stuck' in Hundef1.
+    contradict Hok.
+    apply nonfinal_stuck_state_goes_wrong; auto.
+Qed.
+
+Lemma die_is_bsim : forall dinfo Cfg1 St1 Cfg2 St2
+  (Hnuse: used_in_fdef (DI_id dinfo) (DI_f dinfo) = false)
+  (Hwfcfg: OpsemPP.wf_Config Cfg1) (Hwfpp: OpsemPP.wf_State Cfg1 St1)
+  (Hsim: State_simulation dinfo Cfg1 St1 Cfg2 St2)
+  (Hok: ~ sop_goeswrong Cfg1 St1)
+  St2' tr2 (Hop2: Opsem.sInsn Cfg2 St2 St2' tr2)
+  (Hwfcfg2: OpsemPP.wf_Config Cfg2) (Hwfpp2: OpsemPP.wf_State Cfg2 St2),
+  exists St1',
+    Opsem.sop_plus Cfg1 St1 St1' tr2 /\
+    State_simulation dinfo Cfg1 St1' Cfg2 St2'.
+Proof.
+  intros.
+  eapply die_is_bsim_removable_steps in Hsim; eauto.
+  destruct Hsim as [St1' [Hopstar [Hstsim Hnrm]]].
+  eapply die_is_bsim_unremovable_step in Hstsim; eauto 2 using
+      (@OpsemPP.preservation_star DGVs), sop_goeswrong__star.
+  destruct Hstsim as [FS1 [Hopplus1 Hstsim]].
+  exists FS1.
+  split; auto.
+    rewrite <- E0_left. 
+    eapply OpsemProps.sop_star_plus__implies__sop_plus; eauto.
+    apply OpsemProps.sInsn__implies__sop_plus; auto.
+Qed.
+
+Lemma s_isFinialState__die_State_simulation_r2l:
+  forall diinfo cfg1 FS1 cfg2 FS2 r2
+  (Hnuse: used_in_fdef (DI_id diinfo) (DI_f diinfo) = false)
+  (Hwfcfg: OpsemPP.wf_Config cfg1) (Hwfpp: OpsemPP.wf_State cfg1 FS1)
+  (Hstsim : State_simulation diinfo cfg1 FS1 cfg2 FS2)
+  (Hok: ~ sop_goeswrong cfg1 FS1)
+  (Hfinal: Opsem.s_isFinialState cfg2 FS2 = ret r2),
+  exists FS1', 
+    Opsem.sop_star cfg1 FS1 FS1' E0 /\
+    State_simulation diinfo cfg1 FS1' cfg2 FS2 /\
+  exists r1,
+    Opsem.s_isFinialState cfg1 FS1' = ret r1 /\ result_match r1 r2.
+Proof.
+  intros.
+  eapply die_is_bsim_removable_steps in Hstsim; eauto.
+  destruct Hstsim as [FS1' [Hopstar [Hstsim Hnrm]]].
+  exists FS1'.
+  split; auto.
+  split; auto.
+    eapply s_isFinialState__die_State_simulation_r2l' in Hstsim; 
+      eauto using (@OpsemPP.preservation_star DGVs).
+Qed.
+
+Ltac undefined_state__State_simulation_r2l_tac1 :=
+  match goal with
+  | Hstsim: State_simulation _ _ ?St1 _ ?St2 |- _ =>
+    destruct St2 as [[|[? ? [|CurCmds] [] ?] [|[]]] ?]; try tauto;
+    destruct CurCmds; try tauto;
+    destruct St1 as [ECS ?];
+    destruct Hstsim as [X [? [Hstsim [? [? ?]]]]]; subst;
+    inv X;
+    destruct ECS as [|[] ECS]; try tauto;
+    destruct Hstsim as [Hstsim Hstsim'];
+    destruct ECS as [|[] ECS]; try tauto;
+    destruct Hstsim as [? [Htmn [? [? [? [? [? Hstsim]]]]]]]; subst;
+    destruct Hstsim' as [Hstsim' _];
+    destruct Hstsim' as [? [? [? [? [? [? [? Hstsim']]]]]]]; subst;
+   simpl
+  end.
+
+Ltac undefined_state__State_simulation_r2l_tac3 :=
+  match goal with
+  | Hstsim: State_simulation _ _ ?St1 _ ?St2 |- _ =>
+    destruct St2 as [[|[? [? ? ? tmn] CurCmds tmn' ?] ?] ?]; try tauto;
+    destruct tmn; try tauto;
+    destruct CurCmds; try tauto;
+    destruct tmn'; try tauto;
+    destruct St1 as [ECS ?];
+    destruct Hstsim as [X [? [Hstsim [? [? H3]]]]]; subst;
+    inv X;
+    destruct ECS as [|[] ECS]; try tauto;
+    destruct Hstsim as [Hstsim _];
+    destruct Hstsim as [? [Htmn [? [? [? [? [? Hstsim]]]]]]]; subst;
+    let l5 := fresh "l5" in
+    destruct H3 as [l5 [ps5 [cs5 EQ]]]; subst
+  end.
+
+Ltac undefined_state__State_simulation_r2l_tac41 :=
+  match goal with
+  | Hstsim: State_simulation _ _ ?St1 ?cfg2 ?St2 |- _ =>
+    destruct St1 as [ECS ?];
+    destruct Hstsim as [X [? [Hstsim [? [? ?]]]]]; subst;
+    inv X;
+    destruct ECS as [|[? ? ? ? Locals0] ECS]; try tauto;
+    destruct Hstsim as [Hstsim _];
+    destruct Hstsim as [? [? [? [? [H4 [H5 [? Hstsim]]]]]]]; subst
+  end. 
+
+Ltac undefined_state__d_State_simulation_r2l_tac43 := 
+      match goal with
+      | Hstsim: cmds_simulation _ _ _ (_::_) |- _ =>
+      eapply RemoveSim.cmds_simulation_cons_inv' in Hstsim; eauto; subst;
+      destruct Hstsim as [c1' [J2 J3]]; subst
+     end.
+
+Ltac undefined_state__d_State_simulation_r2l_tac42 v' := 
+match goal with
+| Hwfcfg1: OpsemPP.wf_Config ?cfg1, Hwfpp1: OpsemPP.wf_State ?cfg1 ?St1, 
+  H2: ret ?gn = Opsem.getOperandValue ?td v' ?Locals ?fs2,
+  _: reg_simulation _ ?f ?Locals0 ?Locals,
+  _: block_simulation _ ?f ?b _,
+  H4: exists _:_, exists _:_, exists _:_, ?b = _ |- _ =>
+    let G := fresh "G" in
+    let gvs := fresh "gvs" in
+    let EQ := fresh "EQ" in
+    assert (exists gvs, Opsem.getOperandValue td
+      v' Locals0 fs2 = Some gvs) as G; try solve [
+      destruct H4 as [l5 [ps2 [cs21 H4]]]; subst;
+      destruct Hwfcfg1 as [_ [Hwfg1 [Hwfs1 HmInS1]]];
+      destruct Hwfpp1 as [_ [[Hreach1 [HbInF1 [HfInPs1 [_ [Hinscope1 _]]]]] _]];
+      inv_mbind;
+      eapply OpsemPP.getOperandValue_inCmdOps_isnt_stuck; eauto 1; simpl; auto
+    ];
+    destruct G as [gvs G]; symmetry in H2;
+    assert (gvs = gn) as EQ; try solve [
+      destruct H4 as [l1 [ps1 [cs11 H4]]]; subst;
+      destruct Hwfpp1 as [_ [[_ [HbInF1 [HfInPs1 _]]] _]];
+      match goal with
+      | H1 : Opsem.getOperandValue _ v' ?Locals0 _ = ret _ |- _ =>
+        erewrite simulation__getOperandValue in H1; try solve [
+          eauto 2 | value_doesnt_use_did_tac
+        ];
+        uniq_result; auto
+      end
+    ]; subst
+end.
+
+Lemma stacked_frame__unremovable: forall cfg EC1 EC2 ECS Mem0 dinfo
+  (Huniq: uniqEC EC2)
+  (HBinF: match Opsem.CurBB EC1 with 
+   | block_intro _ _ _ (insn_return _ _ _) => True
+   | block_intro _ _ _ (insn_return_void _) => True
+   | _ => False
+   end)
+  (Hwfpp1 : OpsemPP.wf_State cfg
+             {| Opsem.ECS := EC1 :: EC2 :: ECS; Opsem.Mem := Mem0 |}),
+  ~ removable_State dinfo
+     {| Opsem.ECS := EC2 :: ECS; Opsem.Mem := Mem0 |}.
+Proof.
+  intros.
+  destruct Huniq as [J1 [J2 J3]].
+  destruct J3 as [l1 [ps0 [cs0 J3]]]; subst.
+  destruct EC1, EC2; simpl in *. destruct cfg. destruct CurTargetData.
+  destruct Hwfpp1 as 
+     [_ [[_ [HbInF1 [_ [_ [_ _]]]]] [_ Hiscall]]].
+  apply Hiscall in HbInF1.
+  destruct CurBB as [? ? ? []]; tinv HBinF;
+    destruct CurCmds0 as [|[]]; try solve [
+      inv HbInF1 |
+      simpl; destruct_if; destruct_if;
+      eapply dont_remove_impure_cmd with (dinfo:=dinfo) in J2; 
+        eauto using in_middle; simpl; auto;
+      simpl in J2; tauto
+    ].
+Qed.
+
+Lemma undefined_state__die_State_simulation_r2l': forall dinfo cfg1 St1 cfg2
+  St2 (Hstsim : State_simulation dinfo cfg1 St1 cfg2 St2) maxb
+  (Hwfgl: genericvalues_inject.wf_globals maxb (OpsemAux.Globals cfg1))  
+  (Hnuse: used_in_fdef (DI_id dinfo) (DI_f dinfo) = false)
+  (Hwfcfg1: OpsemPP.wf_Config cfg1) (Hwfpp1: OpsemPP.wf_State cfg1 St1) 
+  (Hnrem: ~removable_State dinfo St1) 
+  (Hundef: OpsemPP.undefined_state cfg2 St2),
+  OpsemPP.undefined_state cfg1 St1.
+Proof.
+  unfold removable_State.
+  intros.
+  assert (HuniqECs:=Hwfpp1). apply wf_State__uniqECs in HuniqECs; auto.
+  unfold OpsemPP.undefined_state in Hundef.
+  destruct cfg2 as [S2 [los2 nts2] gl2 fs2].
+  destruct cfg1 as [S1 [los1 nts1] gl1 fs1].
+  repeat match goal with
+  | Hundef : _ \/ _ |- _ => destruct Hundef as [Hundef | Hundef]
+  end.
+  Case "1".
+
+    undefined_state__State_simulation_r2l_tac1.
+    eapply RemoveSim.cmds_simulation_nil_inv' in Hstsim; eauto; subst.
+    assert (Hnrem' : ~
+          removable_State dinfo
+            {|
+            Opsem.ECS := {|
+                            Opsem.CurFunction := CurFunction2;
+                            Opsem.CurBB := CurBB2;
+                            Opsem.CurCmds := CurCmds1;
+                            Opsem.Terminator := Terminator;
+                            Opsem.Locals := Locals2;
+                            Opsem.Allocas := Allocas0 |} :: ECS;
+            Opsem.Mem := Mem |}).
+      clear - Hwfpp1 H3 HuniqECs.
+      destruct H3 as [l5 [ps5 [cs5 H5]]]; subst.
+      eapply stacked_frame__unremovable; eauto; simpl; auto; find_uniqEC.
+    eapply RemoveSim.cmds_simulation_cons_inv' in Hnrem'; eauto.
+    destruct Hnrem' as [cs1' [J1 J3]]; subst. auto.
+
+  Case "2".
+    undefined_state__State_simulation_r2l_tac1.
+    eapply RemoveSim.cmds_simulation_nil_inv' in Hstsim; eauto; subst.
+    assert (Hnrem' : ~
+          removable_State dinfo
+            {|
+            Opsem.ECS := {|
+                            Opsem.CurFunction := CurFunction2;
+                            Opsem.CurBB := CurBB2;
+                            Opsem.CurCmds := CurCmds1;
+                            Opsem.Terminator := Terminator;
+                            Opsem.Locals := Locals2;
+                            Opsem.Allocas := Allocas0 |} :: ECS;
+            Opsem.Mem := Mem |}).
+      clear - Hwfpp1 H3 HuniqECs.
+      destruct H3 as [l5 [ps5 [cs5 H5]]]; subst.
+      eapply stacked_frame__unremovable; eauto; simpl; auto; find_uniqEC.
+    eapply RemoveSim.cmds_simulation_cons_inv' in Hnrem'; eauto.
+    destruct Hnrem' as [cs1' [J1 J3]]; subst.
+    right. left. 
+    destruct Hundef as [Hundef | Hundef]; auto.
+
+  Case "3".
+    undefined_state__State_simulation_r2l_tac3.
+    eapply RemoveSim.cmds_simulation_nil_inv' in Hstsim; eauto; subst.
+    right. right. left. auto.
+
+  Case "4".
+    right; right; right; left.
+    destruct St2 as [[|[? ? [|[] CurCmds] tmn' Locals] ?] ?]; try solve [
+      tauto |
+      inv_mbind; destruct Hundef as [gn [EQ Hundef]]; inv EQ; inv_mbind;
+      undefined_state__State_simulation_r2l_tac41;
+      undefined_state__d_State_simulation_r2l_tac43;
+      undefined_state__d_State_simulation_r2l_tac42 value5; 
+      repeat fill_ctxhole; exists gn; split; auto;
+      fill_ctxhole; auto
+    ].
+
+  Case "5".
+    right. right. right. right. left.
+    destruct St2 as [[|[? ? [|[] CurCmds] tmn' ?] ?] ?]; try tauto.
+    inv_mbind; destruct Hundef as [gn [EQ Hundef]]; inv EQ; inv_mbind.
+    undefined_state__State_simulation_r2l_tac41.
+    undefined_state__d_State_simulation_r2l_tac43.
+    undefined_state__d_State_simulation_r2l_tac42 value5.
+    repeat fill_ctxhole; exists gn. split; auto.
+    fill_ctxhole; auto.
+   
+  Case "6".
+    right. right. right. right. right. left.
+    destruct St2 as [[|[? ? [|[] CurCmds] tmn' ?] ?] ?]; try tauto.
+    inv_mbind; destruct Hundef as [gvs [EQ Hundef]]; inv EQ; inv_mbind.
+    undefined_state__State_simulation_r2l_tac41.
+    undefined_state__d_State_simulation_r2l_tac43. 
+    undefined_state__d_State_simulation_r2l_tac42 value1.
+    repeat fill_ctxhole; exists gvs. split; auto.
+    fill_ctxhole; auto.
+
+  Case "7".
+    right. right. right. right. right. right. left.
+    destruct St2 as [[|[? ? [|[] CurCmds] tmn' ?] ?] ?]; try tauto.
+    inv_mbind; destruct Hundef as [gv [mgv [EQ1 [EQ2 Hundef]]]]; 
+      inv EQ1; inv EQ2; inv_mbind.
+    undefined_state__State_simulation_r2l_tac41.
+    undefined_state__d_State_simulation_r2l_tac43. 
+    undefined_state__d_State_simulation_r2l_tac42 value1.
+    undefined_state__d_State_simulation_r2l_tac42 value2.
+    repeat fill_ctxhole; exists gv; exists mgv.
+    split; auto.
+    fill_ctxhole; auto.
+
+  Case "8".
+    destruct St2 as [[|[? ? [|[] CurCmds] tmn' ?] ?] ?]; try tauto.
+    right; right; right; right. right. right. right.
+    undefined_state__State_simulation_r2l_tac41.
+    inv_mbind.
+    destruct Hundef as [fptr [EQ Hundef]]; inv EQ.
+    inv_mbind.
+    eapply RemoveSim.cmds_simulation_cons_inv' in Hstsim; subst; eauto.
+    destruct Hstsim as [cs2' [J1 J2]]; subst.
+    undefined_state__d_State_simulation_r2l_tac42 value0.
+    repeat fill_ctxhole.
+    exists fptr. split; auto.
+    remember (OpsemAux.lookupExFdecViaPtr gl2 FunTable fptr) as R.
+    destruct R as [[[]]|].
+      inv_mbind.
+      destruct Hundef as [gvs0 [EQ' Hundef]].
+      dgvs_instantiate_inv.
+      assert (exists gvs, 
+                Opsem.params2GVs (los2,nts2) params5 Locals0 fs2 = Some gvs) as G'.
+        destruct H4 as [l5 [ps2 [cs21 H4]]]; subst.
+        destruct Hwfcfg1 as [_ [Hwfg1 [Hwfs1 HmInS1]]];
+        destruct Hwfpp1 as [_ [[Hreach1 [HbInF1 [HfInPs1 [_ [Hinscope1 _]]]]] _]].
+        inv_mbind.
+        eapply OpsemPP.params2GVs_isnt_stuck; eauto 1; simpl; auto.
+          exists nil. auto.
+      destruct G' as [gvs' G'].
+      assert (gvs' = l1) as EQ2.
+        erewrite reg_simulation__params2GVs in G'; eauto.  
+          symmetry_ctx. uniq_result. auto.
+
+          destruct H4 as [l5 [ps1 [cs11 H4]]]; subst;
+          destruct Hwfcfg1 as [_ [Hwfg1 [Hwfs1 HmInS1]]];
+          destruct Hwfpp1 as [_ [[Hreach1 [HbInF1 [HfInPs1 [_ [Hinscope1 _]]]]] _]];
+          eapply conditional_used_in_fdef__used_in_params; destruct dinfo; eauto 1.
+      subst.
+      repeat fill_ctxhole.
+      erewrite TopSim.lookupFdefViaPtr__simulation_None_l2r; eauto.
+      erewrite TopSim.lookupExFdecViaPtr__simulation_r2l; eauto.
+      simpl.
+      exists l1. split; auto.
+        destruct (callExternalOrIntrinsics (los2, nts2) fs2 Mem id0 typ0
+               (args2Typs args5) deckind5 l1) as [[[]]|]; auto.
+        remember (Opsem.exCallUpdateLocals (los2, nts2) typ5 noret5 id5 o Locals) 
+          as R.
+        destruct R; tinv Hundef.
+          unfold Opsem.exCallUpdateLocals in *.
+          destruct_if.
+          destruct o; auto.
+          destruct (fit_gv (los2, nts2) typ5 g); auto.
+            congruence.
+    
+      erewrite TopSim.lookupFdefViaPtr__simulation_None_l2r; eauto.
+      erewrite TopSim.lookupExFdecViaPtr__simulation_None_r2l; eauto.
+Qed.
+
+Lemma undefined_state__die_State_simulation_r2l: forall dinfo cfg1 St1 cfg2 maxb
+  (Hwfgl: genericvalues_inject.wf_globals maxb (OpsemAux.Globals cfg1))  
+  (Hnuse: used_in_fdef (DI_id dinfo) (DI_f dinfo) = false)
+  (Hwfcfg1: OpsemPP.wf_Config cfg1) (Hwfpp1: OpsemPP.wf_State cfg1 St1) 
+  St2 (Hstsim : State_simulation dinfo cfg1 St1 cfg2 St2)
+  (Hundef: OpsemPP.undefined_state cfg2 St2)
+  (Hok: ~ sop_goeswrong cfg1 St1),
+  exists St1',
+    Opsem.sop_star cfg1 St1 St1' E0 /\
+    State_simulation dinfo cfg1 St1' cfg2 St2 /\
+    OpsemPP.undefined_state cfg1 St1'.
+Proof.
+  intros.
+  eapply die_is_bsim_removable_steps in Hstsim; eauto.
+  destruct Hstsim as [FS1' [Hopstar [Hstsim Hnrm]]].
+  exists FS1'. 
+  split; auto.
+  split; auto.
+    eapply undefined_state__die_State_simulation_r2l' in Hstsim; 
+      eauto using (@OpsemPP.preservation_star DGVs).
+Qed.
+
+Lemma sop_star__die_State_simulation: forall diinfo cfg1 IS1 cfg2 IS2 tr FS2 
+  (Hwfpp1: OpsemPP.wf_State cfg1 IS1) (Hwfcfg1: OpsemPP.wf_Config cfg1)
+  (Hwfpp2: OpsemPP.wf_State cfg2 IS2) (Hwfcfg2: OpsemPP.wf_Config cfg2) maxb
+  (Hwfg: genericvalues_inject.wf_globals maxb (OpsemAux.Globals cfg1))
+  (Hless: 0 <= maxb) (Hnuse: used_in_fdef (DI_id diinfo) (DI_f diinfo) = false)
+  (Hstsim : State_simulation diinfo cfg1 IS1 cfg2 IS2)
+  (Hopstar : Opsem.sop_star cfg2 IS2 FS2 tr) (Hok: ~ sop_goeswrong cfg1 IS1),
+  exists FS1, Opsem.sop_star cfg1 IS1 FS1 tr /\
+    State_simulation diinfo cfg1 FS1 cfg2 FS2.
+Proof.
+  intros.
+  generalize dependent cfg1.
+  generalize dependent IS1.
+  induction Hopstar; intros.
+    exists IS1. split; auto.
+
+    assert (forall IS1'
+            (Hok' : ~ sop_goeswrong cfg1 IS1')
+            (Hwfpp': OpsemPP.wf_State cfg1 IS1')
+            (Hnrm': ~ removable_State diinfo IS1')
+            (Hstsim' : State_simulation diinfo cfg1 IS1' cfg2 state1),
+            exists FS1 : Opsem.State,
+              Opsem.sop_star cfg1 IS1' FS1 (tr1 ** tr2) /\
+              State_simulation diinfo cfg1 FS1 cfg2 state3) as W1.
+      clear - H Hopstar IHHopstar Hwfcfg1 Hless Hwfg Hnuse Hwfcfg2
+              Hwfpp2. 
+      intros.
+      assert (Hwfpp2':=H). apply OpsemPP.preservation in Hwfpp2'; auto.
+      eapply die_is_bsim in H; eauto 2.
+      destruct H as [St1' [Hplus1 Hstsim]].
+      eapply IHHopstar in Hstsim;
+        eauto using (@OpsemPP.preservation_plus DGVs), sop_goeswrong__plus.
+      destruct Hstsim as [FS1 [Hopstar1 Hstsim]].
+      exists FS1.
+      split; auto.
+        eapply OpsemProps.sop_star_trans; eauto.
+        apply OpsemProps.sop_plus__implies__sop_star; eauto.
+
+    eapply die_is_bsim_removable_steps in Hstsim;
+      eauto using (@OpsemPP.preservation_plus DGVs), sop_goeswrong__plus.
+    destruct Hstsim as [St1' [Hopstar1 [Hstsim Hnrm]]].
+    eapply OpsemPP.preservation_star in Hwfpp1; eauto.
+    eapply sop_goeswrong__star in Hok; eauto.
+    eapply W1 in Hstsim; eauto.
+    destruct Hstsim as [FS1 [Hopstar'' Hstsim]].
+    exists FS1.
+    split; auto.
+      clear - Hopstar1 Hopstar''.
+      rewrite <- E0_left.
+      eapply OpsemProps.sop_star_trans; eauto.
+Qed.
+
+Lemma sop_plus__die_State_simulation: forall dinfo cfg1 IS1 cfg2 IS2 tr
+  FS2 maxb
+  (Hwfpp1: OpsemPP.wf_State cfg1 IS1) (Hwfcfg1: OpsemPP.wf_Config cfg1)
+  (Hwfpp2: OpsemPP.wf_State cfg2 IS2) (Hwfcfg2: OpsemPP.wf_Config cfg2)
+  (Hwfg: genericvalues_inject.wf_globals maxb (OpsemAux.Globals cfg1))
+  (Hless: 0 <= maxb) (Hnuse: used_in_fdef (DI_id dinfo) (DI_f dinfo) = false)
+  (Hstsim : State_simulation dinfo cfg1 IS1 cfg2 IS2)
+  (Hopplus : Opsem.sop_plus cfg2 IS2 FS2 tr) (Hok: ~ sop_goeswrong cfg1 IS1),
+  exists FS1, Opsem.sop_plus cfg1 IS1 FS1 tr /\
+    State_simulation dinfo cfg1 FS1 cfg2 FS2.
+Proof.
+  intros.
+  inv Hopplus.
+  assert (Hwfpp2':=H). apply OpsemPP.preservation in Hwfpp2'; auto.
+  eapply die_is_bsim with (Cfg1:=cfg1) in H; eauto.
+  destruct H as [St1' [Hplus1 Hstsim']].
+  eapply sop_star__die_State_simulation in Hstsim'; eauto using
+    (@OpsemPP.preservation_plus DGVs), sop_goeswrong__plus.
+  destruct Hstsim' as [FS1 [Hopstar Hstsim']].
+  exists FS1.
+  split; auto.
+    eapply OpsemProps.sop_plus_star__implies__sop_plus; eauto.
+Qed.
+
+Lemma sop_div__die_State_simulation: forall dinfo cfg1 IS1 cfg2 IS2 tr maxb
+  (Hwfpp1: OpsemPP.wf_State cfg1 IS1) (Hwfcfg1: OpsemPP.wf_Config cfg1)
+  (Hwfpp2: OpsemPP.wf_State cfg2 IS2) (Hwfcfg2: OpsemPP.wf_Config cfg2)
+  (Hwfg: genericvalues_inject.wf_globals maxb (OpsemAux.Globals cfg1))
+  (Hless: 0 <= maxb) (Hnuse: used_in_fdef (DI_id dinfo) (DI_f dinfo) = false)
+  (Hstsim : State_simulation dinfo cfg1 IS1 cfg2 IS2)
+  (Hdiv : Opsem.sop_diverges cfg2 IS2 tr) (Hok: ~ sop_goeswrong cfg1 IS1),
+  Opsem.sop_diverges cfg1 IS1 tr.
+Proof.
+  cofix CIH.
+  intros.
+  inv Hdiv.
+  eapply sop_plus__die_State_simulation in Hstsim; eauto 1.
+  destruct Hstsim as [FS1 [Hopplus Hstsim']].
+  econstructor; eauto.
+  eapply CIH in Hstsim'; eauto using
+    (@OpsemPP.preservation_plus DGVs), sop_goeswrong__plus.
+Qed.
+
+Lemma die_sim: forall id0 f dinfo los nts Ps1 Ps2 main VarArgs
+  (HwfS: wf_system [module_intro los nts (Ps1 ++ product_fdef f :: Ps2)])
+  (Hok: defined_program [module_intro los nts (Ps1 ++ product_fdef f :: Ps2)]
+          main VarArgs)
+  (Heq1: f = DI_f dinfo) (Heq2: id0 = DI_id dinfo),
+  program_sim
+    [module_intro los nts
+      (Ps1 ++  product_fdef (remove_fdef id0 f) :: Ps2)]
+    [module_intro los nts (Ps1 ++ product_fdef f :: Ps2)]
+    main VarArgs.
+Proof.
+  intros. subst.
+  assert (Hnuse: used_in_fdef (DI_id dinfo) (DI_f dinfo) = false).  
+    destruct dinfo. auto.
+  assert (Huniq:=HwfS). apply wf_system__uniqSystem in Huniq; auto.
+  assert (system_simulation dinfo
+    [module_intro los nts (Ps1 ++ product_fdef (DI_f dinfo) :: Ps2)]
+    [module_intro los nts
+      (Ps1 ++ product_fdef (remove_fdef (DI_id dinfo) (DI_f dinfo)) :: Ps2)])
+    as Hssim.
+    constructor; auto.
+    repeat split; auto.
+    simpl in Huniq. destruct Huniq as [[_ [_ Huniq]] _].
+    unfold TopSim.products_simulation. simpl. unfold system_simulation.
+    apply uniq_products_simulation; auto.
+
+Ltac die_sim_init :=
+match goal with
+| H: Opsem.s_genInitState [module_intro ?los ?nts _] _ _ _ = Some (?cfg, ?IS)
+  |- _ =>
+    assert (OpsemPP.wf_Config cfg /\ OpsemPP.wf_State cfg IS) as Hwfst';
+      try solve [eapply s_genInitState__opsem_wf in H; eauto using die_wfS];
+    eapply s_genInitState__die_State_simulation in H; eauto;
+    destruct H as [maxb [cfg1 [IS1 [Hinit1 [Hstsim [Hwfg Hless]]]]]];
+    assert (OpsemPP.wf_Config cfg1/\ OpsemPP.wf_State cfg1 IS1) as Hwfst;
+      try solve [eapply s_genInitState__opsem_wf; eauto]
+end.
+
+Ltac die_sim_end :=
+ match goal with
+| Hstsim' : State_simulation ?dinfo ?cfg1 ?FS1 ?cfg ?FS,
+  Hopstar1 : Opsem.sop_star ?cfg1 _ ?FS1 _ |- _ =>
+    assert (OpsemPP.wf_State cfg FS) as Hwfst''; 
+      try solve [eapply OpsemPP.preservation_star; eauto; try tauto];
+    assert (OpsemPP.wf_State cfg1 FS1) as Hwfst1'';
+      try solve [eapply OpsemPP.preservation_star; eauto; try tauto]
+end.
+
+  constructor; auto.
+    intros tr t Hconv.
+    inv Hconv.
+    die_sim_init.
+    eapply sop_star__die_State_simulation in Hstsim;
+      eauto using defined_program__doesnt__go_wrong; try tauto.
+    destruct Hstsim as [FS1 [Hopstar1 Hstsim']].
+    die_sim_end.
+    eapply s_isFinialState__die_State_simulation_r2l in Hstsim'; 
+      eauto using sop_goeswrong__star, defined_program__doesnt__go_wrong; try tauto.
+    destruct Hstsim' 
+      as [FS1' [Hopstar1' [Hstsim'' [r1 [Hfinal Hrmatch]]]]].
+    assert (Opsem.sop_star cfg1 IS1 FS1' tr) as Hopstar1''.
+      rewrite <- E0_right.
+      eapply OpsemProps.sop_star_trans; eauto.
+    exists r1. 
+    split; auto using result_match_symm. 
+      econstructor; eauto.
+
+    intros tr Hdiv.
+    inv Hdiv.
+    die_sim_init.
+    eapply sop_div__die_State_simulation in Hstsim; 
+      try solve [eauto using defined_program__doesnt__go_wrong| tauto].
+    destruct Hstsim as [FS1 Hopdiv1].
+    econstructor; eauto.
+
+    intros tr t Hgowrong.
+    inv Hgowrong.
+    assert (OpsemPP.wf_Config cfg /\ OpsemPP.wf_State cfg t) as HwfSt.
+      eapply s_genInitState__opsem_wf in H; eauto using die_wfS.
+      destruct H as [Hcfg2 HwfSt2].
+      apply OpsemPP.preservation_star in H0; auto.
+    assert (OpsemPP.undefined_state cfg t) as Hundef.
+      apply stuck__undefined_state in H2; try solve [auto | tauto].
+    die_sim_init.
+    eapply sop_star__die_State_simulation in Hstsim; eauto;
+      eauto using defined_program__doesnt__go_wrong; try tauto.
+    destruct Hstsim as [FS1 [Hopstar1 Hstsim']].
+    die_sim_end.
+    assert (Hundef':=Hundef).
+    eapply undefined_state__die_State_simulation_r2l in Hundef'; 
+      try solve [eauto using sop_goeswrong__star, defined_program__doesnt__go_wrong | 
+                 tauto].
+    destruct Hundef' as [FS1' [Hopstar2 [Hsim Hundef']]].
+    assert (Opsem.s_isFinialState cfg1 FS1' = merror) as Hfinal'.
+      apply OpsemPP.preservation_star in Hopstar2; auto; try tauto.
+      eapply s_isFinialState__die_State_simulation_None_r2l in H2; 
+        try solve [eauto | tauto].
+    apply undefined_state__stuck' in Hundef'.
+    exists (tr**E0). exists FS1'.
+    econstructor; eauto using (@OpsemProps.sop_star_trans DGVs).   
+Qed.
+
