src3.0/Transforms/die_wfS.v
@@ -1,0 +1,37 @@
+Require Import vellvm.
+Require Import Kildall.
+Require Import ListSet.
+Require Import Maps.
+Require Import Lattice.
+Require Import Iteration.
+Require Import primitives.
+Require Import program_sim.
+Require Import palloca_props.
+Require Import die.
+
+Lemma die_wfS: forall id0 f diinfo los nts Ps1 Ps2
+  (HwfS: wf_system [module_intro los nts (Ps1 ++ product_fdef f :: Ps2)])
+  (Heq1: f = DI_f diinfo) (Heq2: id0 = DI_id diinfo),
+  wf_system 
+    [module_intro los nts (Ps1 ++  product_fdef (remove_fdef id0 f) :: Ps2)].
+Admitted.
+
+Lemma subst_fdef__diinfo: forall f id0 v0,
+  exists diinfo:DIInfo, DI_f diinfo = subst_fdef id0 v0 f /\ DI_id diinfo = id0.
+Admitted.
+
+Lemma die_wfPI: forall id0 f diinfo los nts Ps1 Ps2 pinfo
+  (Hwfpi: WF_PhiInfo pinfo)
+  (HwfS: wf_system [module_intro los nts (Ps1 ++ product_fdef f :: Ps2)])
+  (Heq1: f = DI_f diinfo) (Heq2: id0 = DI_id diinfo) (Heq3: f = PI_f pinfo),
+  WF_PhiInfo (update_pinfo pinfo (remove_fdef id0 f)).
+Admitted.
+
+Lemma remove_successors : forall f id',
+  successors f = successors (remove_fdef id' f).
+Admitted.
+
+Lemma remove_reachablity_analysis : forall f id',
+  reachablity_analysis f = reachablity_analysis (remove_fdef id' f).
+Admitted.
+
